wp with steps

theories/gitree/weakestpre.v
@@ -166,8 +166,8 @@ Section ucmra.
 
 End ucmra.
 
-Section weakestpre.
-  Context {n : nat} {a : is_ctx_dep} (rs : gReifiers a n) {A} `{!Cofe A}.
+Section state.
+  Context {n : nat} {a : is_ctx_dep} (rs : gReifiers a n) A `{!Cofe A}.
   Notation rG := (gReifiers_sReifier rs).
   Notation F := (sReifier_ops rG).
   Notation IT := (IT F A).
@@ -177,15 +177,6 @@ Section weakestpre.
   Notation stateR := (gReifiers_ucmra rs IT).
   Let of_state := (of_state rs IT).
   Let of_idx := (of_idx rs IT).
-  Notation reify := (reify rG).
-  Notation internal_step := (internal_step rG).
-  Notation internal_steps := (internal_steps rG).
-  Notation tp_internal_step := (tp_internal_step rG).
-  Notation tp_internal_steps := (tp_internal_steps rG).
-  Notation external_step := (external_step rG).
-  Notation external_steps := (external_steps rG).
-  Notation tp_external_step := (tp_external_step rG).
-  Notation tp_external_steps := (tp_external_steps rG).
 
   Implicit Type op : opid F.
   Implicit Type α β : IT.
@@ -280,7 +271,75 @@ Section weakestpre.
   #[export] Instance subG_stateΣ {Σ} : subG stateΣ Σ → statePreG Σ.
   Proof. solve_inG. Qed.
 
-  Context `{!invGS Σ} `{!stateG Σ}.
+End state.
+
+Arguments state_interp {_ _ _ _ _ _ _}.
+Arguments has_state_idx {_ _ _ _ _ _ _}.
+Arguments has_substate {_ _ _ _ _ _ _ _ _}.
+Arguments state_interp_has_state_idx_update {_ _ _ _ _}.
+Arguments state_interp_has_state_idx_agree {_ _ _ _ _}.
+Arguments new_state_interp {_ _ _ _ _}.
+
+Section GS.
+  Context {n : nat} {a : is_ctx_dep} (rs : gReifiers a n) A `{!Cofe A}.
+  Notation rG := (gReifiers_sReifier rs).
+  Notation F := (sReifier_ops rG).
+  Notation IT := (IT F A).
+  Notation ITV := (ITV F A).
+  Notation stateF := (gReifiers_state rs).
+  Notation stateO := (stateF ♯ IT).
+  Notation stateR := (gReifiers_ucmra rs IT).
+
+  Class gitreeGS_gen (Σ : gFunctors) :=
+    GitreeG {
+        #[global] gitreeInvGS :: invGS Σ;
+        #[global] gitreeStateGS :: stateG rs A Σ;
+        state_interp_fun : nat → stateO → iProp Σ;
+        aux_interp_fun : nat → iProp Σ;
+        fork_post : ITV -> iProp Σ;
+        #[global] fork_post_ne :: NonExpansive fork_post;
+        num_later_per_step : nat → nat;
+        state_interp_fun_mono n σ :
+        state_interp_fun n σ ⊢ |={∅}=> state_interp_fun (S n) σ;
+        #[global] state_interp_fun_ne n :: NonExpansive (state_interp_fun n);
+        state_interp_fun_decomp n σ :
+        state_interp_fun n σ ⊣⊢ aux_interp_fun n ∗ state_interp σ;
+      }.
+End GS.
+
+Arguments gitreeInvGS {_ _ _ _ _ _ _}.
+Arguments gitreeStateGS {_ _ _ _ _ _ _}.
+Arguments state_interp_fun {_ _ _ _ _ _ _}.
+Arguments fork_post {_ _ _ _ _ _ _}.
+Arguments num_later_per_step {_ _ _ _ _ _ _}.
+Arguments aux_interp_fun {_ _ _ _ _ _ _}.
+
+Section weakestpre.
+  Context {n : nat} {a : is_ctx_dep} (rs : gReifiers a n) {A} `{!Cofe A}.
+  Notation rG := (gReifiers_sReifier rs).
+  Notation F := (sReifier_ops rG).
+  Notation IT := (IT F A).
+  Notation ITV := (ITV F A).
+  Notation stateF := (gReifiers_state rs).
+  Notation stateO := (stateF ♯ IT).
+  Notation stateR := (gReifiers_ucmra rs IT).
+  Let of_state := (of_state rs IT).
+  Let of_idx := (of_idx rs IT).
+  Notation reify := (reify rG).
+  Notation internal_step := (internal_step rG).
+  Notation internal_steps := (internal_steps rG).
+  Notation tp_internal_step := (tp_internal_step rG).
+  Notation tp_internal_steps := (tp_internal_steps rG).
+  Notation external_step := (external_step rG).
+  Notation external_steps := (external_steps rG).
+  Notation tp_external_step := (tp_external_step rG).
+  Notation tp_external_steps := (tp_external_steps rG).
+
+  Implicit Type op : opid F.
+  Implicit Type α β : IT.
+
+  Context `{!gitreeGS_gen rs A Σ}.
+
   Notation iProp := (iProp Σ).
   Notation coPsetO := (leibnizO coPset).
 
@@ -292,26 +351,50 @@ Section weakestpre.
     : (ITV -d> iProp) -n> coPsetO -n> IT -n> iProp
     := λne Φ E α,
       ((∃ αv, IT_to_V α ≡ Some αv ∧ |={E}=> Φ αv)
-       ∨ (IT_to_V α ≡ None ∧ ∀ σ,
-            state_interp σ
+       ∨ (IT_to_V α ≡ None ∧ ∀ σ ns,
+            state_interp_fun ns σ
             ={E,∅}=∗ ((∃ α' σ' en, internal_step α σ α' σ' en)
                       ∨ (∃ e, α ≡ Err e ∧ ⌜s e⌝))
             ∧ (∀ σ' β en, internal_step α σ β σ' en
-                          -∗ £ 1
-                          ={∅}▷=∗ |={∅,E}=>
-                 state_interp σ'
+                          -∗ £ (S (num_later_per_step ns))
+                          ={∅}▷=∗^(S $ num_later_per_step ns) |={∅,E}=>
+                 state_interp_fun (S ns) σ'
                  ∗ self Φ E β
-                 ∗ [∗ list] i ↦ ef ∈ en, self (λne _, True) ⊤ ef)))%I.
+                 ∗ [∗ list] i ↦ ef ∈ en, self fork_post ⊤ ef)))%I.
   Next Obligation. solve_proper. Qed.
-  Next Obligation. solve_proper. Qed.
-  Next Obligation. intros ?????? [] ?; simpl; solve_proper. Qed.
-  Next Obligation. solve_proper. Qed.
+  Next Obligation.
+    intros ?????? H ?; simpl.
+    f_equiv; first solve_proper.
+    f_equiv.
+    do 2 (f_equiv; intros ?).
+    f_equiv.
+    solve_proper_prepare.
+    rewrite H.
+    f_equiv.
+  Qed.
+  Next Obligation.
+    intros ?????? [] ?; simpl.
+    f_equiv; first solve_proper.
+    f_equiv.
+    f_equiv; intros ?.
+    f_equiv; intros p.
+    do 3 f_equiv.
+    do 3 (f_equiv; intros ?).
+    do 5 f_equiv.
+    induction (num_later_per_step p).
+    - solve_proper.
+    - solve_proper.
+  Qed.
 
   #[local] Instance wp_pre_contractive s : Contractive (wp_pre s).
   Proof.
     unfold wp_pre.
-    intros m s1 s2 Hs Φ1 E1 a'. simpl.
-    solve_contractive.
+    intros m s1 s2 Hs Φ1 E1 a'; simpl.
+    do 20 (f_contractive || f_equiv).
+    induction num_later_per_step as [| k IH]; simpl.
+    - solve_contractive.
+    - rewrite -IH.
+      solve_contractive.
   Qed.
 
   Definition wp α s E Φ := fixpoint (wp_pre s) Φ E α.
@@ -320,15 +403,15 @@ Section weakestpre.
     wp α s E' Φ ≡
        ((∃ αv, IT_to_V α ≡ Some αv ∧ |={E'}=> Φ αv)
         ∨ (IT_to_V α ≡ None
-           ∧ ∀ σ, state_interp σ
+           ∧ ∀ σ ns, state_interp_fun ns σ
                   ={E',∅}=∗ ((∃ α' σ' en, internal_step α σ α' σ' en)
                              ∨ (∃ e, α ≡ Err e ∧ ⌜s e⌝))
                   ∧ (∀ σ' β en, internal_step α σ β σ' en
-                                -∗ £ 1
-                                ={∅}▷=∗ |={∅,E'}=>
-                       state_interp σ'
+                                -∗ £ (S (num_later_per_step ns))
+                                ={∅}▷=∗^(S $ num_later_per_step ns) |={∅,E'}=>
+                       state_interp_fun (S ns) σ'
                        ∗ wp β s E' Φ
-                       ∗ [∗ list] i ↦ ef ∈ en, wp ef s ⊤ (λne _, True))))%I.
+                       ∗ [∗ list] i ↦ ef ∈ en, wp ef s ⊤ fork_post)))%I.
   Proof.
     rewrite /wp (fixpoint_unfold (wp_pre s) Φ E' α) //.
   Qed.
@@ -361,23 +444,29 @@ Section weakestpre.
     rewrite !wp_unfold.
     f_equiv; first by repeat f_equiv.
     f_equiv; first  solve_proper.
-    f_equiv. f_equiv. f_equiv.
+    f_equiv. f_equiv.
+    f_equiv; intros ?.
+    f_equiv.
     f_equiv.
     f_equiv; first solve_proper.
-    f_equiv. f_equiv. f_equiv. f_equiv.
-    f_equiv; intros ?.
-    f_equiv; first solve_proper. simpl.
-    f_equiv. f_equiv.
-    f_contractive. f_equiv. f_equiv.
+    do 3 (f_equiv; intros ?).
+    f_equiv; first solve_proper.
     f_equiv.
-    f_equiv.
-    - apply IH; eauto.
-      eapply dist_le; [apply Hp|lia].
-    - do 3 f_equiv.
-      unfold wp.
-      do 3 f_equiv.
-      apply fixpoint_ne.
-      solve_proper.
+    induction num_later_per_step as [| k IH']; simpl.
+    - f_equiv.
+      f_contractive.
+      do 4 f_equiv.
+      + apply IH; eauto.
+        eapply dist_le; [apply Hp|lia].
+      + do 3 f_equiv.
+        unfold wp.
+        do 3 f_equiv.
+        apply fixpoint_ne.
+        solve_proper.
+    - f_equiv.
+      f_equiv.
+      f_equiv.
+      apply IH'.
   Qed.
 
   #[export] Instance wp_proper :
@@ -438,7 +527,7 @@ Section weakestpre.
         iPoseProof (option_equivI with "H") as "H".
         done. }
     iRight. iSplit; eauto.
-    iIntros (σ) "Hs". iMod "H" as "H".
+    iIntros (σ ns) "Hs". iMod "H" as "H".
     iDestruct "H" as "[H|H]".
     - iDestruct "H" as (?) "[H _]".
       iPoseProof (option_equivI with "H") as "H".
@@ -472,17 +561,22 @@ Section weakestpre.
       iExists _. iSplit; eauto. iMod "H" as "H".
       by iApply "H2".
     - iRight. iDestruct "H1" as "[H1 H]".
-      iSplit; first by eauto. iIntros (σ) "Hs".
+      iSplit; first by eauto. iIntros (σ ns) "Hs".
       iMod ("H" with "Hs") as "[$ H]".
       iModIntro. iIntros (σ' β en) "Hst Hlc".
       iMod ("H" with "Hst Hlc") as "H".
       iModIntro. iNext.
       iMod "H" as "H". iModIntro.
-      iMod "H" as "[$ [H G]]".
-      iModIntro.
-      iSplitL "H H2".
-      + by iApply ("IH" with "H").
-      + iFrame.
+      iInduction (num_later_per_step) as [| k IH] "G".
+      + iMod "H" as "[$ [H G]]".
+        iModIntro.
+        iSplitL "H H2".
+        * by iApply ("IH" with "H").
+        * iFrame.
+      + iMod "H" as "H".
+        iModIntro.
+        iNext.
+        iApply ("G" with "H1 H2 H").
   Qed.
 
   Lemma wp_fupd E1 α s Φ : WP α @ s;E1 {{ v, |={E1}=> Φ v }} ⊢ WP α @ s;E1 {{ Φ }}.
@@ -497,22 +591,37 @@ Section weakestpre.
     iIntros "H". rewrite (wp_unfold (Tick _)).
     iRight. iSplit.
     { iPureIntro. apply IT_to_V_Tau. }
-    iIntros (σ) "Hs". iApply fupd_mask_intro; first solve_ndisj.
+    iIntros (σ ns) "Hs".
+    iApply fupd_mask_intro; first solve_ndisj.
     iIntros "Hcl". iSplit.
     - iLeft. iExists α,σ,[]. iLeft. eauto.
     - iIntros (σ' β en) "Hst Hlc". rewrite internal_step_tick.
-      iDestruct "Hst" as "[Hb [Hs' Hen]]".
-      iRewrite "Hs'" in "Hs". iFrame "Hs".
-      iModIntro. iNext. iModIntro.
-      iMod "Hcl" as "_".
-      iModIntro. iRewrite "Hb".
-      iFrame "H".
-      destruct en.
-      + done.
-      + iExFalso.
-        iPoseProof (list_equivI with "Hen") as "Hen".
-        iSpecialize ("Hen" $! 0).
-        by iPoseProof (option_equivI with "Hen") as "Hen".
+      iDestruct "Hst" as "[#Hb [#Hs' #Hen]]".
+      iRewrite "Hs'" in "Hs".
+      iClear "Hs'".
+      iSimpl.
+      iModIntro.
+      iNext.
+      iRewrite - "Hb" in "H".
+      iClear "Hb".
+      iInduction num_later_per_step as [| k IH] "G".
+      + iMod (state_interp_fun_mono with "Hs") as "Hs".
+        iModIntro.
+        iFrame "H".
+        iAssert (⌜en = []⌝)%I as "->".
+        {
+          destruct en; first done.
+          iExFalso.
+          iPoseProof (list_equivI with "Hen") as "Hen'".
+          iSpecialize ("Hen'" $! 0).
+          by iPoseProof (option_equivI with "Hen'") as "Hen''".
+        }
+        iSimpl.
+        iFrame "Hs".
+        iMod "Hcl" as "_".
+        iModIntro. done.
+      + iDestruct "Hlc" as "[Hlc1 Hlc2]".
+        iApply ("G" with "H Hs Hcl Hlc2").
   Qed.
 
   Lemma wp_tick_n α s E1 Φ k :
@@ -527,6 +636,16 @@ Section weakestpre.
 
   Opaque gState_recomp.
 
+  Local Definition wptp s t Φs := ([∗ list] e;Φ ∈ t;Φs, WP e @ s {{ Φ }})%I.
+
+  Local Instance wptp_ne s : NonExpansive2 (wptp s).
+  Proof.
+    intros k x1 x2 Hx Φ1 Φ2 HΦ.
+    rewrite /wptp.
+    apply big_sepL2_ne_2; [done | done |].
+    solve_proper.
+  Qed.
+
   (* We can generalize this based on the stuckness bit *)
   Lemma wp_reify_idx E1 E2 s Φ i (lop : opid (sReifier_ops (rs !!! i))) :
     let op : opid F := (existT i lop) in
@@ -539,7 +658,7 @@ Section weakestpre.
                    ▷ (£ 1 -∗ has_state_idx i σ'
                       -∗ |={E2,E1}=>
                         WP β @ s;E1 {{ Φ }}
-                                 ∗ [∗ list] i ↦ ef ∈ en, WP ef @ s; ⊤ {{ _, True }}))
+                                 ∗ wptp s en (replicate (length en) fork_post) ))
     -∗ WP (Vis op x k) @ s;E1 {{ Φ }}.
   Proof.
     intros op x k.
@@ -547,47 +666,80 @@ Section weakestpre.
     rewrite (wp_unfold (Vis _ _ _)).
     iRight. iSplit.
     { iPureIntro. apply IT_to_V_Vis. }
-    iIntros (fs) "Hgst".
+    iIntros (fs ns) "Hgst".
     destruct (gState_decomp i fs) as [σ0 rest] eqn:Hdecomp.
     assert (fs ≡ gState_recomp rest σ0) as Hfs.
     { symmetry. apply gState_recomp_decomp.
       by rewrite Hdecomp. }
     iMod "H" as (σ σ' β en) "[Hlst H]".
+    (* XXX: fixme, proper typeclass is not picked *)
+    iAssert (state_interp_fun ns fs
+               ≡ state_interp_fun ns (gState_recomp rest σ0))%I as "HEQ".
+    {
+      iApply f_equivI.
+      rewrite Hfs.
+      done.
+    }
     iAssert (σ0 ≡ σ)%I with "[Hlst Hgst]" as "#Hss".
-    { iEval (rewrite Hfs) in "Hgst".
-      iApply (state_interp_has_state_idx_agree with "Hgst Hlst"). }
+    {
+      iRewrite "HEQ" in "Hgst". iClear "HEQ".
+      iDestruct (state_interp_fun_decomp with "Hgst") as "[_ Hgst]".
+      iApply (state_interp_has_state_idx_agree with "Hgst Hlst").
+    }
     iDestruct ("H" $! rest) as "[Hreify H]".
     iRewrite -"Hss" in "Hreify".
     iEval (rewrite -Hfs) in "Hreify".
     iApply fupd_mask_intro; first solve_ndisj.
     iIntros "Hcl2".
     iSplit.
-    { (* it is safe *)
+    {
+      (* it is safe *)
       iLeft.
       iExists β, (gState_recomp rest σ'), en. iRight.
-      iExists op, x, k; eauto. }
+      iExists op, x, k; eauto.
+    }
     iIntros (fs' α0 en0) "Hst Hlc". rewrite internal_step_vis.
     iAssert (gState_recomp rest σ' ≡ fs' ∧ Tick β ≡ Tick α0 ∧ en ≡ en0)%I
       with "[Hreify Hst]" as "[Hst [Hb Hen]]".
-    { iRewrite "Hreify" in "Hst".
+    {
+      iRewrite "Hreify" in "Hst".
       do 2 rewrite prod_equivI; simpl.
       iDestruct "Hst" as "(Hst & G)".
       iFrame "G".
       done.
     }
-    iEval (rewrite Hfs) in "Hgst".
+    iRewrite "HEQ" in "Hgst". iClear "HEQ".
+    iDestruct (state_interp_fun_decomp with "Hgst") as "[Hrest Hgst]".
     iMod (state_interp_has_state_idx_update i σ' with "Hgst Hlst") as "[Hgst Hlst]".
+    iDestruct (state_interp_fun_decomp with "[$Hrest $Hgst]") as "Hgst".
+    iMod (state_interp_fun_mono with "Hgst") as "Hgst".
     iModIntro. iNext. iModIntro.
-    iMod "Hcl2" as "_".
-    iMod ("H" with "Hlc Hlst") as "[H1 H2]".
-    iModIntro. iRewrite -"Hst".
-    iRewrite -"Hb".
-    iFrame "Hgst H1".
-    iApply (internal_eq_rewrite with "Hen");
-      last iExact "H2".
-    intros m t1 t2 H.
-    apply big_opL_ne_2; first done.
-    solve_proper.
+    iAssert (state_interp_fun (S ns) fs')%I with "[Hgst Hst]" as "Hgst".
+    {
+      iAssert (state_interp_fun (S ns) (gState_recomp rest σ')
+                 ≡ state_interp_fun (S ns) fs')%I with "[Hst]" as "HEQ".
+      { by iApply f_equivI. }
+      iRewrite -"HEQ".
+      done.
+    }
+    iInduction num_later_per_step as [| p IH] "J".
+    - iFrame "Hgst".
+      iMod "Hcl2" as "_".
+      iMod ("H" with "Hlc Hlst") as "[H1 H2]".
+      iModIntro.
+      iRewrite -"Hb".
+      iFrame "H1".
+      unfold wptp.
+      rewrite big_sepL2_replicate_r; last done.
+      iApply (internal_eq_rewrite with "Hen");
+        last iExact "H2".
+      intros m t1 t2 H.
+      apply big_opL_ne_2; first done.
+      solve_proper.
+    - iModIntro.
+      iNext.
+      iDestruct "Hlc" as "[Hlc1 Hlc2]".
+      iApply ("J" with "H Hcl2 Hlc2 Hb Hen Hlst Hgst").
   Qed.
 
   Lemma wp_reify  E1 s Φ i (lop : opid (sReifier_ops (rs !!! i)))
@@ -597,7 +749,7 @@ Section weakestpre.
     has_state_idx i σ
     -∗ ▷ (£ 1 -∗ has_state_idx i σ'
           -∗ WP β @ s;E1 {{ Φ }}
-                      ∗ [∗ list] i ↦ ef ∈ en, WP ef @ s; ⊤ {{ _, True }})
+                      ∗ wptp s en (replicate (length en) fork_post))
     -∗ WP (Vis op x k) @ s;E1 {{ Φ }}.
   Proof.
     intros op Hr.
@@ -619,7 +771,7 @@ Section weakestpre.
     rewrite wp_unfold.
     iRight. iSplit.
     { rewrite IT_to_V_Err//. }
-    iIntros (σ) "Hσ". iApply fupd_mask_intro; first set_solver.
+    iIntros (σ ns) "Hσ". iApply fupd_mask_intro; first set_solver.
     iIntros "Hcl".
     iSplit.
     { iRight. eauto with iFrame. }
@@ -638,7 +790,7 @@ Section weakestpre.
     - iLeft. iDestruct "H1" as (av) "[H1 H]".
       iExists _. iSplit; eauto.
     - iRight. iDestruct "H1" as "[H1 H]".
-      iSplit; first by eauto. iIntros (σ) "Hs".
+      iSplit; first by eauto. iIntros (σ ns) "Hs".
       iMod ("H" with "Hs") as "[Hs H]".
       iModIntro. iSplit.
       { iDestruct "Hs" as "[$ | Hs]".
@@ -648,451 +800,261 @@ Section weakestpre.
       iMod ("H" with "Hst Hlc") as "H".
       iModIntro. iNext.
       iMod "H" as "H". iModIntro.
-      iMod "H" as "[$ [G1 G2]]".
-      iModIntro.
-      iSplitL "IH G1".
-      + by iApply ("IH" with "G1").
-      + iInduction en as [| en] "IH'"; first done.
-        rewrite !big_opL_cons.
-        iDestruct "G2" as "[G2 G3]".
-        iSplitL "G2".
-        * by iApply ("IH" with "G2").
-        * by iApply ("IH'" with "[$H1] [$Hs]").
+      iInduction num_later_per_step as [| p IH] "J".
+      + iMod "H" as "[$ [G1 G2]]".
+        iModIntro.
+        iSplitL "IH G1".
+        * by iApply ("IH" with "G1").
+        * iInduction en as [| en] "IH'"; first done.
+          rewrite !big_opL_cons.
+          iDestruct "G2" as "[G2 G3]".
+          iSplitL "G2".
+          -- by iApply ("IH" with "G2").
+          -- by iApply ("IH'" with "[$H1] [$Hs]").
+      + iMod "H" as "H".
+        iModIntro.
+        iNext.
+        iApply ("J" with "H1 Hs H").
   Qed.
 
-  (** "adequacy" statements *)
-  Lemma wp_internal_step α σ β σ' en s Ψ :
-    ⊢ internal_step α σ β σ' en -∗ state_interp σ -∗ WP α @ s {{ Ψ }}
-      -∗ £ 2 ={⊤}=∗ state_interp σ'
-                  ∗ WP β @ s {{ Ψ }}
-                  ∗ [∗ list] ef ∈ en, WP ef @ s {{ λne _ : ITVO, True }}.
+  (** "preservation" statements *)
+  Lemma wp_internal_step_preservation' i α σ β σ' en s Ψ :
+    ⊢ internal_step α σ β σ' en
+      -∗ state_interp_fun i σ
+      -∗ WP α @ s {{ Ψ }}
+      -∗ £ (S (num_later_per_step i))
+      ={⊤,∅}=∗ |={∅}▷=>^(S $ num_later_per_step i) |={∅,⊤}=>
+          state_interp_fun (S i) σ'
+          ∗ WP β @ s {{ Ψ }}
+          ∗ [∗ list] ef ∈ en, WP ef @ s {{ fork_post }}.
   Proof.
-    iIntros "Hstep Hs H [Hlc Hlc']".
+    iIntros "Hstep Hs H Hlc".
     rewrite (wp_unfold α). iDestruct "H" as "[H|[Ha H]]".
     - iExFalso. iDestruct "H" as (αv) "[H _]".
       iApply (internal_step_ITV with "H Hstep").
     - iSpecialize ("H" with "Hs"). iDestruct "H" as "[_ H]".
       iMod "H" as "H".
-      iMod ("H" with "Hstep Hlc'") as "H".
-      iApply (fupd_trans ∅ ∅).
-      iApply (lc_fupd_elim_later with "Hlc").
+      iMod ("H" with "Hstep Hlc") as "H".
+      iModIntro. iModIntro.
       iNext.
       iMod "H" as "H".
-      iMod "H" as "[H1 [H2 H3]]".
       iModIntro.
-      iFrame.
+      iInduction num_later_per_step as [| p IH] "J".
+      + iMod "H" as "[H1 [H2 H3]]".
+        iFrame "H1 H2 H3".
+        by iModIntro.
+      + iMod "H" as "H".
+        iModIntro.
+        iNext.
+        iApply ("J" with "Ha H").
   Qed.
 
-  Lemma wp_internal_steps α σ β σ' en m s Ψ :
-    ⊢ internal_steps α σ β σ' en m -∗ state_interp σ -∗ WP α @ s {{ Ψ }}
-      -∗ £ (3 * m) ={⊤}=∗ state_interp σ'
-                        ∗ WP β @ s {{ Ψ }}
-                        ∗ [∗ list] ef ∈ en, WP ef @ s {{ λne _ : ITVO, True }}.
+  Lemma wp_internal_step_preservation i α σ β σ' en s Ψ :
+    ⊢ internal_step α σ β σ' en
+      -∗ aux_interp_fun i
+      -∗ state_interp σ
+      -∗ WP α @ s {{ Ψ }}
+      -∗ £ (S (num_later_per_step i))
+      ={⊤,∅}=∗ |={∅}▷=>^(S $ num_later_per_step i) |={∅,⊤}=>
+          aux_interp_fun (S i)
+          ∗ state_interp σ'
+          ∗ WP β @ s {{ Ψ }}
+          ∗ [∗ list] ef ∈ en, WP ef @ s {{ fork_post }}.
   Proof.
-    iIntros "Hstep Hs H [Hlc Hlc']".
-    iInduction m as [| m] "IH" forall (α σ en).
-    - rewrite internal_steps_0.
-      iDestruct "Hstep" as "(H1 & H2 & H3)".
-      iRewrite "H1" in "H".
-      iRewrite "H2" in "Hs".
-      iModIntro.
-      iFrame "Hs H".
-      iApply (internal_eq_rewrite _ _ with "[H3]");
-        [| iApply internal_eq_sym; iExact "H3" |].
-      + intros m x1 x2 Hx. apply big_opL_ne_2; first done.
-        solve_proper.
-      + by rewrite big_opL_nil.
-    - rewrite internal_steps_S.
-      rewrite lc_succ.
-      iDestruct "Hlc" as "(Hlcone & Hlcrest)".
-      rewrite !Nat.add_0_r.
-      iEval (rewrite lc_split lc_succ) in "Hlc'".
-      iDestruct "Hlc'" as "((Hlcone'' & Hlcrest'') & Hlcone' & Hlcrest')".
-      iDestruct "Hstep" as "(%γ & %σ'' & %l' & %l'' & H1 & H2 & H3)".
-      iCombine "Hlcone' Hlcone''" as "Hlctwo".
-      iMod (wp_internal_step with "H2 Hs H Hlctwo") as "(G1 & G2 & G3)".
-      iDestruct (lc_fupd_elim_later ⊤ with "Hlcone H3") as "G4".
-      iSpecialize ("IH" $! γ σ'' l'' with "G4 G1 G2 Hlcrest").
-      rewrite lc_split.
-      iSpecialize ("IH" with "[$Hlcrest' $Hlcrest'']").
-      do 2 iMod "IH".
-      iModIntro.
-      iDestruct "IH" as "(IH1 & IH2 & IH3)".
-      iFrame "IH1 IH2".
-      iApply (internal_eq_rewrite _ _ with "[H1]");
-        [| iApply internal_eq_sym; iExact "H1" |].
-      + intros k x1 x2 Hx. apply big_opL_ne_2; first done.
-        solve_proper.
-      + rewrite big_opL_app.
-        by iFrame "G3 IH3".
-  Qed.
-
-  Lemma wp_tp_internal_step αs σ βs σ' s Ψs :
-    ⊢ tp_internal_step αs σ βs σ' -∗ state_interp σ
-      -∗ ([∗ list] x;Ψ ∈ αs;Ψs, WP x @ s {{ Ψ }})
-      -∗ ∀ βs' βs'',
-    βs ≡ βs' ++ βs''
-    -∗ length βs' ≡ length αs
-    -∗ £ 2 ={⊤}=∗ state_interp σ'
-                ∗ ([∗ list] x;Ψ ∈ βs';Ψs, WP x @ s {{ Ψ }})
-                ∗ ([∗ list] x ∈ βs'', WP x @ s {{ constO True }}).
-  Proof.
-    iIntros "Hstep Hs H %βs' %βs'' #Heq %Hlen Hlc".
-    iDestruct "Hstep" as "(%α0 & %α1 & %γ & %γ' & %en & #H1 & #H2 & Hstep)".
-    iAssert ([∗ list] x;Ψ ∈ (α0 ++ γ :: α1);Ψs, WP x @ s {{ Ψ }})%I with "[H]" as "H".
-    {
-      iApply (internal_eq_rewrite _ _ (λ y, [∗ list] x;Ψ ∈ y;Ψs, WP x @ s {{ Ψ }})%I
-               with "H1");
-        last iExact "H".
-      intros k x1 x2 Hx.
-      apply big_sepL2_ne_2; first done.
-      - reflexivity.
-      - solve_proper.
-    }
-    iDestruct (big_sepL2_app_inv_l with "H") as "(%l2 & %l2' & %Ψl & G1 & G2)".
-    iDestruct (big_sepL2_cons_inv_l with "G2") as "(%x2 & %l2'' & %HEQ & G2 & G3)".
-    iDestruct (wp_internal_step with "Hstep Hs G2 Hlc") as "G4".
-    iMod "G4" as "(G4 & G5 & G6)".
+    iIntros "Hstep Haux Hs H Hlc".
+    iDestruct (state_interp_fun_decomp with "[$Hs $Haux]") as "Hs".
+    iMod (wp_internal_step_preservation' with "Hstep Hs H Hlc") as "H".
     iModIntro.
-    iFrame "G4".
-    iAssert (βs'' ≡ en)%I as "HEQ''".
-    {
-      iRewrite "Heq" in "H2".
-      iPoseProof (f_equivI (drop (length βs')) with "H2") as "H3".
-      rewrite drop_app_length Hlen.
-      iAssert (length αs ≡ length (α0 ++ γ' :: α1))%I as "H4".
-      {
-        iRewrite "H1".
-        rewrite !app_length /=.
-        iApply (f_equivI (plus (length α0))).
-        done.
-      }
-      iRewrite "H4" in "H3".
-      rewrite {2} app_comm_cons.
-      rewrite app_assoc drop_app drop_all app_nil_l.
-      rewrite Nat.sub_diag drop_0.
-      iDestruct (f_equivI (drop (length (α0 ++ γ' :: α1))) with "H2") as "H5".
-      iDestruct (internal_eq_sym with "H5") as "H6"; iClear "H5".
-      rewrite drop_app.
-      rewrite Nat.sub_diag drop_0.
-      rewrite drop_all app_nil_l.
-      iRewrite - "H4" in "H6".
-      rewrite -Hlen.
-      rewrite drop_app drop_all app_nil_l Nat.sub_diag drop_0.
-      done.
-    }
-    iSplitL "G1 G5 G3".
-    {
-      iAssert (βs' ≡ α0 ++ γ' :: α1)%I as "HEQ'".
-      {
-        iRewrite "Heq" in "H2".
-        iDestruct (f_equivI (take (length βs')) with "H2") as "H3".
-        rewrite take_app Nat.sub_diag take_0 app_nil_r firstn_all.
-        rewrite Hlen.
-        iRewrite "H1" in "H3".
-        rewrite {2} app_comm_cons app_assoc.
-        rewrite take_app.
-        iAssert (length (α0 ++ γ :: α1) ≡ length (α0 ++ γ' :: α1))%I as "H4".
-        {
-          iPureIntro.
-          by rewrite !app_length /=.
-        }
-        iRewrite "H4" in "H3".
-        rewrite firstn_all Nat.sub_diag take_0 app_nil_r.
-        done.
-      }
-      iApply (internal_eq_rewrite _ _ (λ y, [∗ list] x;Ψ ∈ y;Ψs, WP x @ s {{ Ψ }})%I
-               with "[HEQ']");
-        [| iApply internal_eq_sym; iExact "HEQ'" |].
-      {
-        intros k y1 y2 Hy.
-        by apply big_sepL2_ne_2; [| done | solve_proper].
-      }
-      rewrite Ψl.
-      iApply (big_sepL2_app with "G1").
-      rewrite HEQ.
-      iApply (big_sepL2_cons with "[-]").
-      iFrame "G5 G3".
-    }
-    {
-      iApply (internal_eq_rewrite _ _ (λ y, [∗ list] x ∈ y, WP x @ s {{ constO True }})%I
-               with "[HEQ'']");
-        [| iApply internal_eq_sym; iExact "HEQ''" |].
-      {
-        intros k y1 y2 Hy.
-        apply big_opL_ne_2; first solve_proper.
-        repeat intros; solve_proper.
-      }
-      iFrame "G6".
-    }
+    iInduction num_later_per_step as [| p IH] "J".
+    - iMod "H" as "H".
+      iModIntro.
+      iNext.
+      iMod "H" as "H".
+      iModIntro.
+      iMod "H" as "(H1 & H2 & H3)".
+      iModIntro.
+      iFrame "H2 H3".
+      iApply (state_interp_fun_decomp with "H1").
+    - iMod "H" as "H".
+      iModIntro.
+      iNext.
+      iApply "J".
+      iApply "H".
   Qed.
 
-  Lemma tp_internal_steps_decomp αs βs σ σ' k :
-    ⊢ £ k -∗ tp_internal_steps αs σ βs σ' k
-      ={⊤}=∗ ∃ β1 β2 : listO IT, βs ≡ β1 ++ β2 ∗ length αs ≡ length β1.
+  Local Lemma wptp_internal_step_preservation' αs σ βs σ' ns s Φs :
+    tp_internal_step αs σ βs σ'
+    -∗ state_interp_fun ns σ
+    -∗ £ (S (num_later_per_step ns))
+    -∗ wptp s αs Φs
+    -∗ ∃ nt', |={⊤,∅}=> |={∅}▷=>^(S $ num_later_per_step ns) |={∅,⊤}=>
+          state_interp_fun (S ns) σ' ∗
+            wptp s βs (Φs ++ replicate nt' fork_post).
   Proof.
-    iInduction k as [| k] "IH" forall (αs σ); iIntros "Hlc H".
+    iIntros "Hstep Hσ Hcred Ht".
+    iDestruct "Hstep" as (α1 α2 γ γ' en) "(HEQ1 & HEQ2 & Hstep)".
+    iExists (length en).
+    iRewrite "HEQ1" in "Ht".
+    iDestruct (big_sepL2_app_inv_l with "Ht") as (Φs1 Φs2 ->) "[H1 Ht]".
+    iDestruct (big_sepL2_cons_inv_l with "Ht") as (Φ Φs3 ->) "[Ht H2]".
+    iMod (wp_internal_step_preservation' with "Hstep Hσ Ht Hcred") as "H". iModIntro.
+    iApply (step_fupdN_wand with "H"). iIntros ">($ & He2 & Hefs) !>".
+    rewrite -(assoc_L app) -app_comm_cons.
+    iRewrite "HEQ2".
+    iFrame "H1 He2 H2".
+    rewrite big_sepL2_replicate_r; done.
+  Qed.
+
+  Local Lemma wptp_internal_step_preservation αs σ βs σ' ns s Φs :
+    tp_internal_step αs σ βs σ'
+    -∗ aux_interp_fun ns
+    -∗ state_interp σ
+    -∗ £ (S (num_later_per_step ns))
+    -∗ wptp s αs Φs
+    -∗ ∃ nt', |={⊤,∅}=> |={∅}▷=>^(S $ num_later_per_step ns) |={∅,⊤}=>
+          aux_interp_fun (S ns) ∗
+          state_interp σ' ∗
+            wptp s βs (Φs ++ replicate nt' fork_post).
+  Proof.
+    iIntros "Hstep Hσ Haux Hcred Ht".
+    iDestruct (state_interp_fun_decomp with "[$Hσ $Haux]") as "Hσ".
+    iDestruct (wptp_internal_step_preservation' with "Hstep Hσ Hcred Ht") as (nt) "H".
+    iExists nt.
+    iMod "H". iModIntro.
+    iApply (step_fupdN_wand with "H").
+    iIntros ">(H1 & H2)".
+    iFrame "H2".
+    iDestruct (state_interp_fun_decomp with "H1") as "(Hσ & Haux)".
+    by iFrame.
+  Qed.
+
+  Local Fixpoint steps_sum (num_later_per_step : nat → nat) (start ns : nat) : nat :=
+    match ns with
+    | O => 0
+    | S ns =>
+        S $ num_later_per_step start + steps_sum num_later_per_step (S start) ns
+    end.
+
+  Local Lemma wptp_internal_steps_preservation' αs σ βs σ' m ns s Φs :
+  tp_internal_steps αs σ βs σ' m
+  -∗ state_interp_fun ns σ
+  -∗ £ (steps_sum num_later_per_step ns m) -∗
+  wptp s αs Φs
+  ={⊤,∅}=∗ |={∅}▷=>^(steps_sum num_later_per_step ns m) |={∅,⊤}=> ∃ nt',
+    state_interp_fun (m + ns) σ'
+    ∗ wptp s βs (Φs ++ replicate nt' fork_post).
+  Proof.
+    revert αs σ βs σ' ns Φs.
+    induction m as [| m IH];
+      intros αs σ βs σ' ns Φs;
+      iIntros "Hsteps Hσ HCred H".
     - rewrite tp_internal_steps_0.
-      iDestruct "H" as "(H1 & _)".
-      iExists βs, [].
+      iDestruct "Hsteps" as "(HEQ1 & HEQ2)".
+      iRewrite "HEQ1" in "H".
+      iRewrite "HEQ2" in "Hσ".
+      iExists 0.
+      iSimpl.
       rewrite app_nil_r.
-      iRewrite "H1".
-      done.
+      iFrame "Hσ H".
+      by iApply fupd_mask_subseteq.
     - rewrite tp_internal_steps_S.
-      iDestruct "H" as "(%t1 & %t2 & G1 & G2)".
-      iDestruct "Hlc" as "(J1 & J2)".
-      iMod (lc_fupd_elim_later ⊤ (tp_internal_steps t1 t2 βs σ' k) with "J1 G2") as "J".
-      iDestruct (tp_internal_step_decomp with "G1") as "(%u1 & %u2 & #G1' & #G2)".
-      iRewrite "G1'" in "J".
-      iMod ("IH" $! (u1 ++ u2) t2 with "J2 J") as "(%p1 & %p2 & K1 & %K2)".
-      iRewrite "K1".
-      iRewrite "G2".
+      iDestruct "Hsteps" as (γ σ'') "(Hstep & Hsteps)".
+      iSimpl in "HCred".
+      iDestruct "HCred" as "(HCred1 & HCred2 & HCred3)".
+      iCombine "HCred1 HCred2" as "HCred1".
+      iDestruct (wptp_internal_step_preservation' with "Hstep Hσ HCred1 H") as (nt') ">H".
+      specialize (IH γ σ'' βs σ' (S ns) (Φs ++ replicate nt' fork_post)).
+      iSimpl.
       iModIntro.
-      iExists (take (length u1) p1), ((drop (length u1) p1) ++ p2).
-      iSplit.
-      + rewrite app_assoc.
-        iApply (f_equivI (flip app p2) with "[]").
-        by rewrite take_drop.
-      + rewrite firstn_length_le; first done.
-        rewrite -K2.
-        rewrite app_length.
-        lia.
+      iApply step_fupdN_S_fupd.
+      rewrite /= step_fupdN_add.
+      iMod "H".
+      iApply step_fupdN_S_fupd.
+      iSimpl.
+      iModIntro.
+      iNext.
+      iMod "H".
+      iModIntro.
+      iApply (step_fupdN_wand with "H").
+      iIntros ">(H1 & H2)".
+      iDestruct (IH with "Hsteps H1 HCred3 H2") as ">IH".
+      iModIntro.
+      iApply (step_fupdN_wand with "IH"). iIntros ">IH".
+      iDestruct "IH" as (nt'') "[??]".
+      rewrite -app_assoc -replicate_add.
+      rewrite Nat.add_succ_r.
+      iExists _.
+      iFrame.
+      by iApply fupd_mask_subseteq.
   Qed.
 
-  (* k too many credits, but i ain't greedy *)
-  Lemma wp_tp_internal_steps αs σ βs σ' s Ψs k :
-    ⊢ tp_internal_steps αs σ βs σ' k -∗ state_interp σ
-      -∗ ([∗ list] x;Ψ ∈ αs;Ψs, WP x @ s {{ Ψ }})
-      -∗ ∀ βs' βs'',
-    βs ≡ βs' ++ βs''
-    -∗ length βs' ≡ length αs
-    -∗ £ (k * k + 2 * k) ={⊤}=∗ state_interp σ' ∗
-                        ([∗ list] x;Ψ ∈ βs';Ψs, WP x @ s {{ Ψ }})
-                      ∗ ([∗ list] x ∈ βs'', WP x @ s {{ constO True }}).
+  Local Lemma wptp_internal_steps_preservation αs σ βs σ' m ns s Φs :
+  tp_internal_steps αs σ βs σ' m
+  -∗ aux_interp_fun ns
+  -∗ state_interp σ
+  -∗ £ (steps_sum num_later_per_step ns m) -∗
+  wptp s αs Φs
+  ={⊤,∅}=∗ |={∅}▷=>^(steps_sum num_later_per_step ns m) |={∅,⊤}=> ∃ nt',
+    aux_interp_fun (m + ns)
+    ∗ state_interp σ'
+    ∗ wptp s βs (Φs ++ replicate nt' fork_post).
   Proof.
-    iInduction k as [| k] "IH" forall (αs βs σ Ψs); iIntros "Hstep Hs H %βs' %βs'' #HEQ %Hlen Hlc".
-    - rewrite tp_internal_steps_0.
-      iModIntro.
-      iDestruct "Hstep" as "(#H1 & H2)".
-      iRewrite - "H2".
-      iFrame "Hs".
-      iAssert (βs'' ≡ [])%I as "HEQ'".
-      {
-        iDestruct (f_equivI (drop (length βs')) with "HEQ") as "H2".
-        rewrite Hlen.
-        rewrite -{2} Hlen.
-        iRewrite "H1" in "H2".
-        rewrite drop_app Nat.sub_diag drop_0 drop_all.
-        rewrite drop_all app_nil_l.
-        iApply internal_eq_sym.
-        done.
-      }
-      iSplitL "H".
-      {
-        iDestruct (internal_eq_rewrite _ _
-                     (λ y,
-                       ([∗ list] x;Ψ ∈ y;Ψs, WP x @ s {{ Ψ }}))%I
-                    with "[H1 HEQ HEQ'] H") as "H2".
-        {
-          intros m y1 y2 Hy.
-          apply big_sepL2_ne_2; [| reflexivity | solve_proper].
-          by rewrite Hy.
-        }
-        {
-          iRewrite "H1".
-          iRewrite "HEQ".
-          iRewrite "HEQ'".
-          rewrite app_nil_r.
-          iPureIntro.
-          reflexivity.
-        }
-        iExact "H2".
-      }
-      {
-        iApply (internal_eq_rewrite _ _
-                     (λ y,
-                       ([∗ list] x ∈ y, WP x @ s {{ constO True }}))%I
-                    with "[HEQ']").
-        {
-          intros m y1 y2 Hy.
-          apply big_opL_ne_2; first done.
-          solve_proper.
-        }
-        {
-          iApply internal_eq_sym; iExact "HEQ'".
-        }
-        done.
-      }
-    - rewrite tp_internal_steps_S.
-      iPoseProof (big_sepL2_alt with "H") as "HT".
-      iDestruct "HT" as "[%HT1 HT2]".
-      iPoseProof (big_sepL2_alt (λ _ x y, WP x @ s {{ y }}%I) with "[HT2]") as "H".
-      {
-        iSplit; first (iPureIntro; apply HT1).
-        iApply "HT2".
-      }
-      iDestruct "Hstep" as "(%γ & %σ'' & #H1 & H2)".
-      iDestruct (tp_internal_step_decomp with "H1") as "(%γs' & %γs'' & F1 & %F2)".
-      iDestruct (wp_tp_internal_step with "H1 Hs H") as "H3".
-      iClear "H1".
-      iSpecialize ("H3" $! γs' γs'' with "F1 []").
-      { by rewrite F2. }
-      rewrite /= lc_succ plus_n_Sm Nat.add_0_r Nat.mul_succ_r.
-      iDestruct "Hlc" as "[Hlc1 [[Hlc2 [Hlc4 Hlc5]] [Hlc6 [Hlc7 [Hlc8 Hlc9]]]]]".
-      iMod (lc_fupd_elim_later ⊤ with "Hlc1 H2") as "#H2".
-      iMod ("H3" with "[Hlc7 Hlc8]") as "(H3 & H4)"; first by iSplitL "Hlc7".
-      set (F := (λ _, True%I) : ITV -d> iProp).
-      iAssert ([∗ list] x;Ψ ∈ (γs' ++ γs'');(Ψs ++ replicate (length γs'') F), WP x @ s {{ Ψ }})%I with "[H4]" as "H5".
-      {
-        iDestruct "H4" as "(H4 & H5)".
-        iApply (big_sepL2_app with "H4").
-        iApply big_sepL2_alt.
-        iSplit.
-        - iPureIntro.
-          by rewrite replicate_length.
-        - iClear "IH HEQ H2 F1".
-          iInduction γs'' as [| x ens] "IH"; first done.
-          iDestruct "H5" as "(H5 & H6)".
-          simpl.
-          iFrame "H5".
-          iApply "IH".
-          iFrame "H6".
-      }
-      iSpecialize ("IH" $! (γs' ++ γs'')
-                     βs σ'' (Ψs ++ replicate (length γs'') F) with "[H2] H3 H5").
-      {
-        iRewrite "F1" in "H2".
-        iFrame "H2".
-      }
-      iMod (tp_internal_steps_decomp with "Hlc2 H2") as "(%a1 & %a2 & #A1 & %A2)".
-      iSpecialize ("IH" $! a1 a2 with "A1 [] [Hlc4 Hlc5 Hlc6]").
-      {
-        rewrite -A2.
-        by iRewrite "F1".
-      }
-      {
-        iSplitL "Hlc4"; first done.
-        iSplitL "Hlc5"; done.
-      }
-      iMod "IH".
-      iModIntro.
-      iDestruct "IH" as "(IH1 & IH2 & IH3)".
-      iFrame "IH1".
-      iPoseProof (big_sepL2_alt with "IH2") as "HP".
-      iDestruct "HP" as "[%HP1 HP2]".
-      iPoseProof (big_sepL2_alt (λ _ x y, WP x @ s {{ y }}%I) with "[HP2]") as "IH2".
-      {
-        iSplit; first (iPureIntro; apply HP1).
-        iApply "HP2".
-      }
-      iAssert ([∗ list] x;Ψ ∈ a2;(replicate (length a2) F), WP x @ s {{ Ψ }})%I with "[IH3]" as "H5".
-      {
-        iApply big_sepL2_alt.
-        iSplit.
-        - iPureIntro.
-          by rewrite replicate_length.
-        - iClear "A1".
-          iInduction a2 as [| x ens] "IH"; first done.
-          iDestruct "IH3" as "(H5 & H6)".
-          simpl.
-          iFrame "H5".
-          iApply "IH".
-          iFrame "H6".
-      }
-      iPoseProof (big_sepL2_app with "IH2 H5") as "IH".
-      rewrite -app_assoc.
-      iDestruct (internal_eq_rewrite _ _
-                (λ y,
-                  ([∗ list] x;x' ∈ y;_, WP x @ s {{ x' }}))%I
-               with "[A1] IH") as "IH".
-      {
-        intros m y1 y2 Hy.
-        apply big_sepL2_ne_2; first done.
-        - solve_proper.
-        - solve_proper.
-      }
-      {
-        iRewrite - "A1".
-        iApply "HEQ".
-      }
-      rewrite HT1 in Hlen.
-      iDestruct (big_sepL2_app_inv with "IH") as "[IH1 IH2]".
-      { by left. }
-      iFrame "IH1".
-      rewrite -replicate_add.
-      iPoseProof (big_sepL2_alt with "IH2") as "HP".
-      iDestruct "HP" as "[%HW1 HW2]".
-      iPoseProof (big_sepL2_alt (λ _ x y, WP x @ s {{ y }}%I) with "[HW2]") as "IH2".
-      {
-        iSplit; first (iPureIntro; apply HW1).
-        iApply "HW2".
-      }
-      iPoseProof (big_sepL2_replicate_r with "IH2") as "HP".
-      {
-        rewrite replicate_length in HW1.
-        done.
-      }
-      iApply "HP".
+    iIntros "Hstep Haux Hσ HCred H".
+    iDestruct (state_interp_fun_decomp with "[$Hσ $Haux]") as "Hσ".
+    iDestruct (wptp_internal_steps_preservation' with "Hstep Hσ HCred H") as ">H".
+    iModIntro.
+    iApply (step_fupdN_wand with "H").
+    iIntros ">(%nt & H1 & H2)".
+    iExists nt.
+    iDestruct (state_interp_fun_decomp with "H1") as "(Hσ & Haux)".
+    iFrame "H2 Hσ Haux".
+    done.
   Qed.
 
-  Lemma wp_external_step α σ β σ' en s Ψ :
+  Lemma wp_external_step_preservation α σ β σ' en i s Ψ :
     external_step α σ β σ' en →
-    state_interp σ ∗ WP α @ s {{ Ψ }}
-    ⊢  £ 2
-       ={⊤}=∗ (state_interp σ'
-               ∗ WP β @ s {{ Ψ }}
-               ∗ ([∗ list] ef ∈ en, WP ef @ s {{ λne _ : ITVO, True }})).
+    state_interp_fun i σ
+    ∗ WP α @ s {{ Ψ }}
+    ∗ £ (S (num_later_per_step i))
+    ={⊤,∅}=∗ |={∅}▷=>^(S $ num_later_per_step i) |={∅,⊤}=>
+          state_interp_fun (S i) σ'
+          ∗ WP β @ s {{ Ψ }}
+          ∗ ([∗ list] ef ∈ en, WP ef @ s {{ fork_post }}).
   Proof.
-    iIntros (Hst) "[Hs HIC]".
+    iIntros (Hst) "[Hs [HIC HCred]]".
     iAssert (internal_step α σ β σ' en) as "Hst".
     { by iApply external_step_internal_step. }
-    iApply (wp_internal_step with "Hst Hs HIC").
+    iApply (wp_internal_step_preservation' with "Hst Hs HIC HCred").
   Qed.
 
-  Lemma wp_external_steps α σ β σ' en k s Ψ :
-    external_steps α σ β σ' en k →
-    state_interp σ ∗ WP α @ s {{ Ψ }}
-    ⊢  £ (3 * k)
-       ={⊤}=∗ (state_interp σ'
-               ∗ WP β @ s {{ Ψ }}
-               ∗ ([∗ list] ef ∈ en, WP ef @ s {{ λne _ : ITVO, True }})).
-  Proof.
-    iIntros (Hst) "[Hs HIC]".
-    iAssert (internal_steps α σ β σ' en k) as "Hst".
-    { by iApply external_steps_internal_steps. }
-    iApply (wp_internal_steps with "Hst Hs HIC").
-  Qed.
-
-  Lemma wp_tp_external_step αs σ βs σ' s Ψs :
+  Lemma wp_tp_external_step_preservation αs σ βs σ' s Ψs ns :
     tp_external_step αs σ βs σ' →
-    state_interp σ ∗ ([∗ list] x;Ψ ∈ αs;Ψs, WP x @ s {{ Ψ }})
-      ⊢  ∀ βs' βs'',
-    βs ≡ βs' ++ βs''
-    -∗ length βs' ≡ length αs
-      -∗ £ 2 ={⊤}=∗ (state_interp σ'
-                     ∗ ([∗ list] x;Ψ ∈ βs';Ψs, WP x @ s {{ Ψ }})
-                     ∗ ([∗ list] x ∈ βs'', WP x @ s {{ constO True }})).
+    state_interp_fun ns σ
+    ∗ £ (S (num_later_per_step ns))
+    ∗ wptp s αs Ψs
+    -∗ ∃ nt', |={⊤,∅}=> |={∅}▷=>^(S $ num_later_per_step ns) |={∅,⊤}=>
+          state_interp_fun (S ns) σ'
+          ∗ wptp s βs (Ψs ++ replicate nt' fork_post).
   Proof.
-    iIntros (Hst) "[Hs HIC]".
+    iIntros (Hst) "[Hs [HIC HCred]]".
     iAssert (tp_internal_step αs σ βs σ') as "Hst".
     { by iApply tp_external_step_tp_internal_step. }
-    iApply (wp_tp_internal_step with "Hst Hs HIC").
+    iApply (wptp_internal_step_preservation' with "Hst Hs HIC HCred").
   Qed.
 
-  Lemma wp_tp_external_steps αs σ βs σ' s Ψs k :
-    tp_external_steps αs σ βs σ' k →
-    state_interp σ ∗ ([∗ list] x;Ψ ∈ αs;Ψs, WP x @ s {{ Ψ }})
-      ⊢  £ (k * k + 2 * k) ={⊤}=∗ (state_interp σ' ∗ ([∗ list] x;Ψ ∈ (take (length αs) βs);Ψs, WP x @ s {{ Ψ }}) ∗ ([∗ list] x ∈ drop (length αs) βs, WP x @ s {{ constO True }})).
+  Lemma wp_tp_external_steps_preservation αs σ βs σ' s Ψs m ns :
+    tp_external_steps αs σ βs σ' m →
+    state_interp_fun ns σ
+    ∗ £ (steps_sum num_later_per_step ns m)
+    ∗ wptp s αs Ψs
+    ={⊤,∅}=∗ |={∅}▷=>^(steps_sum num_later_per_step ns m) |={∅,⊤}=> ∃ nt',
+    state_interp_fun (m + ns) σ'
+    ∗ wptp s βs (Ψs ++ replicate nt' fork_post).
   Proof.
-    iIntros (Hst) "[Hs HIC]".
-    iAssert (tp_internal_steps αs σ βs σ' k) as "Hst".
+    iIntros (Hst) "[Hs [HIC HCred]]".
+    iAssert (tp_internal_steps αs σ βs σ' m) as "Hst".
     { by iApply tp_external_steps_tp_internal_steps. }
-    iPoseProof (wp_tp_internal_steps with "Hst Hs HIC") as "HTTT".
-    iSpecialize ("HTTT" $! (take (length αs) βs) (drop (length αs) βs)).
-    iSpecialize ("HTTT" with "[] []").
-    { iPureIntro. by rewrite take_drop. }
-    { rewrite take_length_le; first done. by eapply tp_external_steps_mono. }
-    iApply "HTTT".
+    iApply (wptp_internal_steps_preservation' with "Hst Hs HIC HCred").
   Qed.
 
   Lemma IT_error_lem α :
@@ -1115,64 +1077,123 @@ Section weakestpre.
         iApply (IT_vis_err_ne with "Ha").
   Qed.
 
-  Lemma wp_external_steps_internal_safe α σ β σ' l k s Ψ :
-    external_steps α σ β σ' l k →
-    state_interp σ ∗ WP α @ s {{ Ψ }}
-      ⊢  £ (3 * k + 2) ={⊤,∅}=∗
-        (⌜is_Some (IT_to_V β)⌝
-           ∨ (∃ β2 σ2 l2, internal_step β σ' β2 σ2 l2)
-           ∨ (∃ e, β ≡ Err e ∧ ⌜s e⌝)).
+  Definition not_stuck α σ s : iProp := (⌜is_Some (IT_to_V α)⌝
+                                 ∨ (∃ β σ' l, internal_step α σ β σ' l)
+                                 ∨ (∃ e, α ≡ Err e ∧ ⌜s e⌝))%I.
+
+  Lemma wp_not_stuck α σ s i Ψ :
+    state_interp_fun i σ
+    ∗ WP α @ s {{ Ψ }}
+    ={⊤, ∅}=∗ not_stuck α σ s.
   Proof.
-    intros Hst. rewrite wp_external_steps//.
-    iIntros "H [Hlc [Hone Htwo]]". iSpecialize ("H" with "Hlc").
-    iMod "H" as "[Hs H]".
-    rewrite wp_unfold. iDestruct "H" as "[[H | [Hb H]] G]".
-    - iLeft. iDestruct "H" as (av) "[H _]".
-      iApply (fupd_mask_weaken ∅); first done.
-      iIntros "_".
-      iModIntro.
-      destruct (IT_to_V β) as [βv|]; first by eauto.
-      iExFalso. iApply (option_equivI with "H").
-    - iPoseProof (IT_error_lem β) as "Heq".
-      iDestruct "Heq" as "[Heq|Heq]".
-      + iDestruct "Heq" as (e) "Heq".
-        iRight. iRight.
-        iSpecialize ("H" with "Hs").
-        iMod ("H") as "[#Hst H]".
-        iDestruct "Hst" as "[Hst|Hst]".
-        {
-          iExFalso. iDestruct "Hst" as (α' σ'0 en') "Hst".
-          iRewrite "Heq" in "Hst".
-          iApply (internal_step_err with "Hst").
-        }
-        iModIntro. done.
+    iIntros "[Hs H]".
+    rewrite wp_unfold.
+    iDestruct "H" as "[[% [H1 H2]] | [H1 H2]]".
+    - iLeft.
+      iMod (fupd_mask_subseteq ∅); first set_solver. iModIntro.
+      destruct (IT_to_V α) as [αv'|].
+      + by rewrite is_Some_alt.
+      + iExFalso. iApply (option_equivI with "H1").
+    - iMod ("H2" $! σ i with "Hs") as "[[H2 | H2] _]".
       + iRight. iLeft.
-        iMod ("H" with "Hs") as "[#Hst H]".
-        iDestruct "Hst" as "[(%t1 & %t2 & %t3 & Hst)|Hst]"; last first.
-        {
-          iExFalso. iDestruct "Hst" as (e') "[Hst ?]".
-          iApply "Heq". eauto with iFrame.
-        }
-        iExists t1, t2, t3.
-        iFrame "Hst".
-        iModIntro.
-        done.
+        by iModIntro.
+      + iRight. iRight.
+        by iModIntro.
   Qed.
 
-  Lemma wp_external_steps_val α σ βv σ' l k s Ψ `{!NonExpansive Ψ} :
-    external_steps α σ (IT_of_V βv) σ' l k →
-    state_interp σ ∗ WP α @ s {{ Ψ }}
-                 ⊢ £ (3*k) ={⊤}=∗ Ψ βv.
+  Lemma wp_internal_step_progress α σ β σ' l s i Ψ :
+    internal_step α σ β σ' l
+    ∗ state_interp_fun i σ
+    ∗ WP α @ s {{ Ψ }}
+    ∗ £ (S (num_later_per_step i))
+    ={⊤,∅}=∗ |={∅}▷=>^(S (num_later_per_step i)) |={∅}=> not_stuck β σ' s.
   Proof.
-    intros Hst. rewrite wp_external_steps //.
-    iIntros "H Hk". iSpecialize ("H" with "Hk").
-    iMod "H" as "[Hs H]".
-    rewrite wp_unfold. iDestruct "H" as "[[H | [Hb H]] G]".
-    - iDestruct "H" as (av) "[H HH]".
-      rewrite IT_to_of_V. iPoseProof (option_equivI with "H") as "H".
-      by iRewrite "H".
-    - rewrite IT_to_of_V.
-      iExFalso. iApply (option_equivI with "Hb").
+    iIntros "(Hstep & Hs & H & Hcred)".
+    iMod (wp_internal_step_preservation' with "Hstep Hs H Hcred") as "J".
+    iModIntro.
+    iApply (step_fupdN_wand with "J").
+    iIntros ">(J1 & H & J2)".
+    iApply (wp_not_stuck with "[$J1 $H]").
+  Qed.
+
+  Lemma wp_tp_internal_steps_progress αs σ e βs σ' m s ns Ψs :
+    e ∈ βs ->
+    tp_internal_steps αs σ βs σ' m
+    ∗ state_interp_fun ns σ
+    ∗ wptp s αs Ψs
+    ∗ £ (steps_sum num_later_per_step ns m)
+    ={⊤,∅}=∗ |={∅}▷=>^(steps_sum num_later_per_step ns m) |={∅}=> not_stuck e σ' s.
+  Proof.
+    iIntros (HIn) "(Hstep & Hs & H & Hcred)".
+    iDestruct (state_interp_fun_decomp with "Hs") as "[Hs Haux]".
+    iMod (wptp_internal_steps_preservation with "Hstep Hs Haux Hcred H") as "J".
+    iModIntro.
+    iApply (step_fupdN_wand with "J").
+    iIntros ">(%nt & J1 & J2 & J3)".
+    eapply elem_of_list_lookup in HIn as [i Hlook].
+    destruct ((Ψs ++ replicate nt fork_post) !! i) as [Φ|] eqn: Hlook2; last first.
+    {
+      rewrite /wptp big_sepL2_alt. iDestruct "J3" as "[%Hlen J3]". exfalso.
+      eapply lookup_lt_Some in Hlook. rewrite Hlen in Hlook.
+      eapply lookup_lt_is_Some_2 in Hlook. rewrite Hlook2 in Hlook.
+      destruct Hlook as [? ?]. naive_solver.
+    }
+    rewrite /wptp.
+    iDestruct (big_sepL2_lookup with "J3") as "Ht"; [done..|].
+    iDestruct (state_interp_fun_decomp with "[$J1 $J2]") as "Hs".
+    by iApply (wp_not_stuck with "[$Ht $Hs]").
+  Qed.
+
+  Lemma wp_internal_steps_val α σ βv σ' l i s Ψ `{!NonExpansive Ψ} :
+    internal_step α σ (IT_of_V βv) σ' l
+    ∗ state_interp_fun i σ
+    ∗ WP α @ s {{ Ψ }}
+    ∗ £ (S (num_later_per_step i))
+    ={⊤,∅}=∗ |={∅}▷=>^(S (num_later_per_step i)) |={∅}=> Ψ βv.
+  Proof.
+    iIntros "(Hstep & Hs & H & Hcred)".
+    iDestruct (wp_internal_step_preservation' with "Hstep Hs H Hcred") as "J".
+    iMod "J".
+    iModIntro.
+    iApply (step_fupdN_wand with "J").
+    iIntros ">(_ & H & _)".
+    iPoseProof (wp_val_inv with "H") as "H".
+    iMod "H".
+    iFrame "H".
+    iMod (fupd_mask_subseteq ∅); first set_solver. by iModIntro.
+  Qed.
+
+  Lemma wptp_postconditions (Φs : list (ITV -d> iProp))
+    (HΦ : Forall (λ f, NonExpansive f) Φs)
+    s m es1 es2 σ1 ns σ2 :
+    tp_internal_steps es1 σ1 es2 σ2 m
+    -∗ state_interp_fun ns σ1
+    -∗ £ (steps_sum num_later_per_step ns m)
+    -∗ wptp s es1 Φs
+    ={⊤,∅}=∗ |={∅}▷=>^(steps_sum num_later_per_step ns m) |={∅,⊤}=> ∃ nt',
+    state_interp_fun (m + ns) σ2
+    ∗ [∗ list] e;Φ ∈ es2;Φs ++ replicate nt' fork_post, from_option Φ True (IT_to_V e).
+  Proof.
+    iIntros "Hstep Hσ Hcred He".
+    iMod (wptp_internal_steps_preservation' with "Hstep Hσ Hcred He") as "Hwp".
+    iModIntro. iApply (step_fupdN_wand with "Hwp").
+    iMod 1 as (nt') "(Hσ & Ht)"; simplify_eq/=.
+    iExists _. iFrame "Hσ".
+    iApply big_sepL2_fupd.
+    iApply (big_sepL2_impl with "Ht").
+    iIntros "!#" (k e Φ ? HH) "Hwp".
+    destruct (IT_to_V e) as [v2|] eqn:He2'.
+    - iMod (wp_val_inv _ v2 with "Hwp") as "J".
+      + assert (Forall (λ f, NonExpansive f) (replicate nt' fork_post)) as GG.
+        { apply Forall_replicate; apply fork_post_ne. }
+        apply (Forall_lookup_1 (λ f, NonExpansive f)
+                 (Φs ++ replicate nt' fork_post) k Φ); last done.
+        apply Forall_app.
+        split; done.
+      + apply IT_of_to_V'. by rewrite He2'.
+      + rewrite He2' /=.
+        by iFrame "J".
+    - by rewrite He2'.
   Qed.
 
   Global Instance upd_ne {X : ofe} E (Φ : X -n> iProp) :
@@ -1195,46 +1216,195 @@ Section weakestpre.
 
 End weakestpre.
 
-Section weakestpre_specific.
+Definition notStuck : stuckness := λ e, False.
+
+Notation "'WP@{' re } α @ s ; E {{ Φ } }" :=
+  (wp re α s E Φ)
+    (at level 20, α, s, Φ at level 200, only parsing) : bi_scope.
+
+Notation "'WP@{' re } α @ s ; E {{ v , Q } }" :=
+  (wp re α s E (λ v, Q))
+    (at level 20, α, s, Q at level 200,
+      format "'[hv' 'WP@{' re }  α  '/' @  s  ;  E  '/' {{  '[' v ,  '/' Q  ']' } } ']'") : bi_scope.
+
+Notation "'WP@{' re } α @  s {{ β , Φ } }" :=
+  (wp re α s ⊤ (λ β, Φ))
+    (at level 20, α, Φ at level 200,
+      format "'WP@{' re }  α  @  s  {{  β ,  Φ  } }") : bi_scope.
+
+Notation "'WP@{' re } α  @  s {{ Φ } }" :=
+  (wp re α s ⊤ Φ)
+    (at level 20, α, Φ at level 200,
+      format "'WP@{' re }  α  @  s  {{  Φ  } }") : bi_scope.
+
+Notation "'WP@{' re } α {{ β , Φ } }" :=
+  (wp re α notStuck ⊤ (λ β, Φ))
+    (at level 20, α, Φ at level 200,
+      format "'WP@{' re }  α  {{  β ,  Φ  } }") : bi_scope.
+
+Notation "'WP@{' re } α {{ Φ } }" :=
+  (wp re α notStuck ⊤ Φ)
+    (at level 20, α, Φ at level 200,
+      format "'WP@{' re }  α  {{  Φ  } }") : bi_scope.
+
+Section weakestpre_ectx_indep.
   Context {n : nat} {A} `{!Cofe A}.
+  Context (rs : (gReifiers NotCtxDep n)).
+  Notation F := (sReifier_ops (gReifiers_sReifier (n := n) rs)).
+  Notation IT := (IT F A).
+  Notation ITV := (ITV F A).
+  Notation stateF := (gReifiers_state).
+  Notation stateO := (stateF rs ♯ IT).
+  Notation stateR := (gReifiers_ucmra rs IT).
+  Let of_state := (of_state rs IT).
+  Let of_idx := (of_idx rs IT).
+  Notation reify := (reify rs).
+  Notation internal_step := (internal_step rs).
+  Notation internal_steps := (internal_steps rs).
+  Notation tp_internal_step := (tp_internal_step rs).
+  Notation tp_internal_steps := (tp_internal_steps rs).
+  Notation external_step := (external_step rs).
+  Notation external_steps := (external_steps rs).
+  Notation tp_external_step := (tp_external_step rs).
+  Notation tp_external_steps := (tp_external_steps rs).
 
-  Notation rG rs := (gReifiers_sReifier (n := n) rs).
-  Notation F rs := (sReifier_ops (rG rs)).
-  Notation IT rs := (IT (F rs) A).
-  Notation ITV rs := (ITV (F rs) A).
-  Notation stateF rs := (gReifiers_state rs).
-  Notation stateO rs := (stateF rs ♯ IT rs).
-  Notation stateR rs := (gReifiers_ucmra rs (IT rs)).
-  Let of_state {a} rs := (of_state (a:=a) rs (IT rs)).
-  Let of_idx {a} rs := (of_idx (a:=a) rs (IT rs)).
-  Notation reify rs := (reify (rG rs)).
-  Notation internal_step rs := (internal_step (rG rs)).
-  Notation internal_steps rs := (internal_steps (rG rs)).
-  Notation tp_internal_step rs := (tp_internal_step (rG rs)).
-  Notation tp_internal_steps rs := (tp_internal_steps (rG rs)).
-  Notation external_step rs := (external_step (rG rs)).
-  Notation external_steps rs := (external_steps (rG rs)).
-  Notation tp_external_step rs := (tp_external_step (rG rs)).
-  Notation tp_external_steps rs := (tp_external_steps (rG rs)).
+  Context `{!gitreeGS_gen rs A Σ}.
 
-  Context `{!invGS Σ}.
   Notation iProp := (iProp Σ).
   Notation coPsetO := (leibnizO coPset).
 
-  Lemma wp_reify_idx_ctx_dep (rs : gReifiers CtxDep n)
-    `{!@stateG _ CtxDep rs A _ Σ} E1 E2 s Φ i
+  Lemma wp_reify_idx_ctx_indep
+    E1 E2 s Φ i
     (lop : opid (sReifier_ops (rs !!! i))) :
-    let op : opid (F rs) := (existT i lop) in
-    forall (x : Ins (F rs op) ♯ IT rs)
-           (k : Outs (F rs op) ♯ IT rs -n> laterO (IT rs)),
+    let op : opid F := (existT i lop) in
+    forall (x : Ins (F op) ♯ IT)
+      (k : Outs (F op) ♯ IT -n> laterO IT),
+    (|={E1,E2}=>  ∃ σ y σ' β l,
+       has_state_idx i σ
+       ∗ sReifier_re (rs !!! i) lop (x, σ) ≡ Some (y, σ', l)
+       ∗ k y ≡ Next β
+       ∗ ▷ (£ 1 -∗ has_state_idx i σ'
+            ={E2,E1}=∗ WP@{rs} β @ s; E1 {{ Φ }}
+               ∗ wptp rs s (listO_map Tau l) (replicate (length (listO_map Tau l)) fork_post)))
+       -∗ WP@{rs} (Vis op x k) @ s; E1 {{ Φ }}.
+  Proof.
+    intros op x k.
+    iIntros "H".
+    iApply wp_reify_idx.
+    iMod "H" as (σ y σ' β l) "[Hlst [Hreify [Hk H]]]".
+    iModIntro. iExists σ, σ', β, (listO_map Tau l).
+    iFrame "Hlst".
+    iIntros (rest).
+    iFrame "H".
+    iAssert (@gReifiers_re _ NotCtxDep rs _ _ op (x, gState_recomp rest σ)
+               ≡ Some (y, gState_recomp rest σ', l))%I
+      with "[Hreify]"  as "Hgreify".
+    { pose proof (@gReifiers_re_idx n NotCtxDep i rs IT) as J.
+      simpl in J.
+      simpl.
+      rewrite J; clear J.
+      iAssert (optionO_map (prodO_map (prodO_map idfun (gState_recomp rest)) idfun)
+                 (sReifier_re (rs !!! i) lop (x, σ))
+                 ≡ optionO_map (prodO_map (prodO_map idfun (gState_recomp rest)) idfun)
+                 (Some (y, σ', l)))%I with "[Hreify]" as "H".
+      - iApply (f_equivI with "Hreify").
+      - simpl. iExact "H".
+    }
+    iPoseProof (reify_vis_eqI_ctx_indep _ _ _ k with "Hgreify") as "Hreify".
+    iRewrite "Hk" in "Hreify".
+    by rewrite -Tick_eq.
+  Qed.
+
+  Lemma wp_subreify_ctx_indep'
+    E1 E2 s Φ sR `{!subReifier sR rs}
+    (op : opid (sReifier_ops sR)) (x : Ins (sReifier_ops sR op) ♯ IT)
+    (k : Outs (F (subEff_opid op)) ♯ IT -n> laterO IT) :
+    (|={E1,E2}=> ∃ σ y σ' β l,
+       has_substate σ
+       ∗ sReifier_re sR op (x, σ) ≡ Some (y, σ', l)
+       ∗ k (subEff_outs y) ≡ Next β
+       ∗ ▷ (£ 1 -∗ has_substate σ'
+         ={E2,E1}=∗ wp rs β s E1 Φ
+        ∗ wptp rs s (listO_map Tau l) (replicate (length (listO_map Tau l)) fork_post)))
+    -∗ wp rs (Vis (subEff_opid op) (subEff_ins x) k) s E1 Φ.
+  Proof.
+    iIntros "H".
+    iApply wp_reify_idx_ctx_indep.
+    iMod "H" as (σ y σ' β l) "[Hlst [Hreify [Hk H]]]".
+    iModIntro.
+    iExists (sR_state σ),(subEff_outs y), (sR_state σ'), β.
+    iExists l.
+    iFrame "Hlst H Hk".
+    by iApply subReifier_reify_idxI_ctx_indep.
+  Qed.
+
+  Lemma wp_subreify_ctx_indep
+    E1 s Φ sR `{!subReifier sR rs}
+    (op : opid (sReifier_ops sR))
+    (x : Ins (sReifier_ops sR op) ♯ IT)
+    (y : Outs (sReifier_ops sR op) ♯ IT)
+    (k : Outs (F (subEff_opid op)) ♯ IT -n> laterO IT)
+    (σ σ' : sReifier_state sR ♯ IT) β l :
+    sReifier_re sR op (x, σ) ≡ Some (y, σ', l) →
+    k (subEff_outs y) ≡ Next β →
+    has_substate σ
+    -∗ ▷ (£ 1 -∗ has_substate σ'
+          -∗ wp rs β s E1 Φ
+           ∗ wptp rs s (listO_map Tau l) (replicate (length (listO_map Tau l)) fork_post))
+    -∗ wp rs (Vis (subEff_opid op) (subEff_ins x) k) s E1 Φ.
+  Proof.
+    intros HSR Hk.
+    iIntros "Hlst H".
+    iApply (wp_reify with "Hlst H").
+    intros rest.
+    rewrite Tick_eq. rewrite -Hk.
+    rewrite reify_vis_eq_ctx_indep //.
+    by apply (subReifier_reify (a := NotCtxDep)).
+  Qed.
+
+End weakestpre_ectx_indep.
+
+Section weakestpre_ectx_dep.
+  Context {n : nat} {A} `{!Cofe A}.
+  Context (rs : (gReifiers CtxDep n)).
+  Notation F := (sReifier_ops (gReifiers_sReifier (n := n) rs)).
+  Notation IT := (IT F A).
+  Notation ITV := (ITV F A).
+  Notation stateF := (gReifiers_state).
+  Notation stateO := (stateF rs ♯ IT).
+  Notation stateR := (gReifiers_ucmra rs IT).
+  Let of_state := (of_state rs IT).
+  Let of_idx := (of_idx rs IT).
+  Notation reify := (reify rs).
+  Notation internal_step := (internal_step rs).
+  Notation internal_steps := (internal_steps rs).
+  Notation tp_internal_step := (tp_internal_step rs).
+  Notation tp_internal_steps := (tp_internal_steps rs).
+  Notation external_step := (external_step rs).
+  Notation external_steps := (external_steps rs).
+  Notation tp_external_step := (tp_external_step rs).
+  Notation tp_external_steps := (tp_external_steps rs).
+
+  Context `{!gitreeGS_gen rs A Σ}.
+
+  Notation iProp := (iProp Σ).
+  Notation coPsetO := (leibnizO coPset).
+
+  Lemma wp_reify_idx_ctx_dep
+    E1 E2 s Φ i
+    (lop : opid (sReifier_ops (rs !!! i))) :
+    let op : opid F := (existT i lop) in
+    forall (x : Ins (F op) ♯ IT)
+      (k : Outs (F op) ♯ IT -n> laterO IT),
     (|={E1,E2}=>
        ∃ σ y σ' β l,
-       has_state_idx rs i σ
+       has_state_idx i σ
        ∗ sReifier_re (rs !!! i) lop (x, σ, k) ≡ Some (y, σ', l)
        ∗ y ≡ Next β
-       ∗ ▷ (£ 1 -∗ has_state_idx rs i σ'
-            ={E2,E1}=∗ wp rs β s E1 Φ
-                     ∗ ([∗ list] ef ∈ listO_map Tau l, wp rs ef s ⊤ (λ _ : ITV rs, True))))
+       ∗ ▷ (£ 1 -∗ has_state_idx i σ'
+            ={E2,E1}=∗
+            wp rs β s E1 Φ
+            ∗ wptp rs s (listO_map Tau l) (replicate (length (listO_map Tau l)) fork_post)))
     -∗ wp rs (Vis op x k) s E1 Φ.
   Proof.
     intros op x k.
@@ -1260,59 +1430,17 @@ Section weakestpre_specific.
     by rewrite -Tick_eq.
   Qed.
 
-  Lemma wp_reify_idx_ctx_indep (rs : gReifiers NotCtxDep n)
-    `{!@stateG _ NotCtxDep rs A _ Σ} E1 E2 s Φ i
-    (lop : opid (sReifier_ops (rs !!! i))) :
-    let op : opid (F rs) := (existT i lop) in
-    forall (x : Ins (F rs op) ♯ IT rs)
-      (k : Outs (F rs op) ♯ IT rs -n> laterO (IT rs)),
-    (|={E1,E2}=>  ∃ σ y σ' β l,
-       has_state_idx rs i σ
-       ∗ sReifier_re (rs !!! i) lop (x, σ) ≡ Some (y, σ', l)
-       ∗ k y ≡ Next β
-       ∗ ▷ (£ 1 -∗ has_state_idx rs i σ'
-            ={E2,E1}=∗ wp rs β s E1 Φ
-                     ∗ ([∗ list] ef ∈ listO_map Tau l, wp rs ef s ⊤ (λ _ : ITV rs, True))))
-    -∗ wp rs (Vis op x k) s E1 Φ.
-  Proof.
-    intros op x k.
-    iIntros "H".
-    iApply wp_reify_idx.
-    iMod "H" as (σ y σ' β l) "[Hlst [Hreify [Hk H]]]".
-    iModIntro. iExists σ, σ', β, (listO_map Tau l).
-    iFrame "Hlst".
-    iIntros (rest).
-    iFrame "H".
-    iAssert (@gReifiers_re _ NotCtxDep rs _ _ op (x, gState_recomp rest σ)
-               ≡ Some (y, gState_recomp rest σ', l))%I
-      with "[Hreify]"  as "Hgreify".
-    { pose proof (@gReifiers_re_idx n NotCtxDep i rs (IT rs)) as J.
-      simpl in J.
-      simpl.
-      rewrite J; clear J.
-      iAssert (optionO_map (prodO_map (prodO_map idfun (gState_recomp rest)) idfun)
-                 (sReifier_re (rs !!! i) lop (x, σ))
-                 ≡ optionO_map (prodO_map (prodO_map idfun (gState_recomp rest)) idfun)
-                 (Some (y, σ', l)))%I with "[Hreify]" as "H".
-      - iApply (f_equivI with "Hreify").
-      - simpl. iExact "H".
-    }
-    iPoseProof (reify_vis_eqI_ctx_indep _ _ _ k with "Hgreify") as "Hreify".
-    iRewrite "Hk" in "Hreify".
-    by rewrite -Tick_eq.
-  Qed.
-
-  Lemma wp_subreify_ctx_dep' (rs : gReifiers CtxDep n)
-    `{!@stateG _ CtxDep rs A _ Σ} E1 E2 s Φ sR `{!subReifier sR rs}
-    (op : opid (sReifier_ops sR)) (x : Ins (sReifier_ops sR op) ♯ (IT rs))
-    (k : Outs (F rs (subEff_opid op)) ♯ IT rs -n> laterO (IT rs)) :
+  Lemma wp_subreify_ctx_dep'
+    E1 E2 s Φ sR `{!subReifier sR rs}
+    (op : opid (sReifier_ops sR)) (x : Ins (sReifier_ops sR op) ♯ IT)
+    (k : Outs (F (subEff_opid op)) ♯ IT -n> laterO IT) :
     (|={E1,E2}=> ∃ σ y σ' β l,
-       has_substate rs σ
+       has_substate σ
        ∗ sReifier_re sR op (x, σ, (k ◎ subEff_outs)) ≡ Some (y, σ', l)
        ∗ y ≡ Next β
-       ∗ ▷ (£ 1 -∗ has_substate rs σ'
+       ∗ ▷ (£ 1 -∗ has_substate σ'
             ={E2,E1}=∗ wp rs β s E1 Φ
-                     ∗ ([∗ list] ef ∈ listO_map Tau l, wp rs ef s ⊤ (λ _ : ITV rs, True))))
+                     ∗ wptp rs s (listO_map Tau l) (replicate (length (listO_map Tau l)) fork_post)))
     -∗ wp rs (Vis (subEff_opid op) (subEff_ins x) k) s E1 Φ.
   Proof.
     iIntros "H".
@@ -1331,39 +1459,17 @@ Section weakestpre_specific.
     by rewrite ofe_iso_12.
   Qed.
 
-  Lemma wp_subreify_ctx_indep' (rs : gReifiers NotCtxDep n)
-    `{!@stateG _ NotCtxDep rs A _ Σ} E1 E2 s Φ sR `{!subReifier sR rs}
-    (op : opid (sReifier_ops sR)) (x : Ins (sReifier_ops sR op) ♯ (IT rs))
-    (k : Outs (F rs (subEff_opid op)) ♯ IT rs -n> laterO (IT rs)) :
-    (|={E1,E2}=> ∃ σ y σ' β l,
-       has_substate rs σ
-       ∗ sReifier_re sR op (x, σ) ≡ Some (y, σ', l)
-       ∗ k (subEff_outs y) ≡ Next β
-       ∗ ▷ (£ 1 -∗ has_substate rs σ'
-            ={E2,E1}=∗ wp rs β s E1 Φ
-                     ∗ ([∗ list] ef ∈ listO_map Tau l, wp rs ef s ⊤ (λ _ : ITV rs, True))))
-    -∗ wp rs (Vis (subEff_opid op) (subEff_ins x) k) s E1 Φ.
-  Proof.
-    iIntros "H".
-    iApply wp_reify_idx_ctx_indep.
-    iMod "H" as (σ y σ' β l) "[Hlst [Hreify [Hk H]]]".
-    iModIntro.
-    iExists (sR_state σ),(subEff_outs y), (sR_state σ'), β.
-    iExists l.
-    iFrame "Hlst H Hk".
-    by iApply subReifier_reify_idxI_ctx_indep.
-  Qed.
-
-  Lemma wp_subreify_ctx_dep (rs : gReifiers CtxDep n)
-    `{!@stateG _ CtxDep rs A _ Σ} E1 s Φ sR `{!subReifier sR rs}
+  Lemma wp_subreify_ctx_dep
+    E1 s Φ sR `{!subReifier sR rs}
     (op : opid (sReifier_ops sR))
-    (x : Ins (sReifier_ops sR op) ♯ IT rs) (y : laterO (IT rs))
-    (k : Outs (F rs (subEff_opid op)) ♯ IT rs -n> laterO (IT rs))
-    (σ σ' : sReifier_state sR ♯ IT rs) β l :
+    (x : Ins (sReifier_ops sR op) ♯ IT) (y : laterO IT)
+    (k : Outs (F (subEff_opid op)) ♯ IT -n> laterO IT)
+    (σ σ' : sReifier_state sR ♯ IT) β l :
     sReifier_re sR op (x, σ, (k ◎ subEff_outs)) ≡ Some (y, σ', l) →
     y ≡ Next β →
-    has_substate rs σ
-    -∗ ▷ (£ 1 -∗ has_substate rs σ' -∗ wp rs β s E1 Φ ∗ ([∗ list] ef ∈ listO_map Tau l, wp rs ef s ⊤ (λ _ : ITV rs, True)))
+    has_substate σ
+    -∗ ▷ (£ 1 -∗ has_substate σ' -∗ wp rs β s E1 Φ
+      ∗ wptp rs s (listO_map Tau l) (replicate (length (listO_map Tau l)) fork_post))
     -∗ wp rs (Vis (subEff_opid op) (subEff_ins x) k) s E1 Φ.
   Proof.
     intros HSR Hk.
@@ -1373,7 +1479,7 @@ Section weakestpre_specific.
     rewrite Tick_eq. rewrite -Hk.
     rewrite reify_vis_eq_ctx_dep //.
     pose proof (@subReifier_reify n CtxDep sR rs _
-                  (IT rs) _ op x y (k ◎ subEff_outs) σ σ' rest) as H'.
+                  (IT) _ op x y (k ◎ subEff_outs) σ σ' rest) as H'.
     simpl in H'.
     rewrite <-H'.
     - simpl.
@@ -1387,28 +1493,29 @@ Section weakestpre_specific.
       reflexivity.
   Qed.
 
-  Lemma wp_subreify_ctx_indep (rs : gReifiers NotCtxDep n)
-    `{!@stateG _ NotCtxDep rs A _ Σ} E1 s Φ sR `{!subReifier sR rs}
-    (op : opid (sReifier_ops sR))
-    (x : Ins (sReifier_ops sR op) ♯ IT rs)
-    (y : Outs (sReifier_ops sR op) ♯ IT rs)
-    (k : Outs (F rs (subEff_opid op)) ♯ IT rs -n> laterO (IT rs))
-    (σ σ' : sReifier_state sR ♯ IT rs) β l :
-    sReifier_re sR op (x, σ) ≡ Some (y, σ', l) →
-    k (subEff_outs y) ≡ Next β →
-    has_substate rs σ
-    -∗ ▷ (£ 1 -∗ has_substate rs σ' -∗ wp rs β s E1 Φ
-                                     ∗ ([∗ list] ef ∈ listO_map Tau l, wp rs ef s ⊤ (λ _ : ITV rs, True)))
-    -∗ wp rs (Vis (subEff_opid op) (subEff_ins x) k) s E1 Φ.
-  Proof.
-    intros HSR Hk.
-    iIntros "Hlst H".
-    iApply (wp_reify with "Hlst H").
-    intros rest.
-    rewrite Tick_eq. rewrite -Hk.
-    rewrite reify_vis_eq_ctx_indep //.
-    by apply (subReifier_reify (a := NotCtxDep)).
-  Qed.
+End weakestpre_ectx_dep.
+
+Section weakestpre_lifting.
+  Context {n : nat} {A} `{!Cofe A}.
+
+  Notation rG rs := (gReifiers_sReifier (n := n) rs).
+  Notation F rs := (sReifier_ops (rG rs)).
+  Notation IT rs := (IT (F rs) A).
+  Notation ITV rs := (ITV (F rs) A).
+  Notation stateF rs := (gReifiers_state rs).
+  Notation stateO rs := (stateF rs ♯ IT rs).
+  Notation stateR rs := (gReifiers_ucmra rs (IT rs)).
+  Let of_state {a} rs := (of_state (a:=a) rs (IT rs)).
+  Let of_idx {a} rs := (of_idx (a:=a) rs (IT rs)).
+  Notation reify rs := (reify (rG rs)).
+  Notation internal_step rs := (internal_step (rG rs)).
+  Notation internal_steps rs := (internal_steps (rG rs)).
+  Notation tp_internal_step rs := (tp_internal_step (rG rs)).
+  Notation tp_internal_steps rs := (tp_internal_steps (rG rs)).
+  Notation external_step rs := (external_step (rG rs)).
+  Notation external_steps rs := (external_steps (rG rs)).
+  Notation tp_external_step rs := (tp_external_step (rG rs)).
+  Notation tp_external_steps rs := (tp_external_steps (rG rs)).
 
   Global Instance subEffCtxIndep a (rs : gReifiers a n)
     sR
@@ -1419,7 +1526,8 @@ Section weakestpre_specific.
   Defined.
 
   Lemma wp_subreify_ctx_indep_lift (rs : gReifiers CtxDep n)
-    `{!@stateG _ CtxDep rs A _ Σ} E1 s Φ sR
+    `{gitreeGS_gen n _ rs A Σ}
+    E1 s Φ sR
     `{!subReifier (sReifier_NotCtxDep_CtxDep sR) rs}
     (op : opid (sReifier_ops sR))
     (x : Ins (sReifier_ops sR op) ♯ IT rs)
@@ -1428,10 +1536,10 @@ Section weakestpre_specific.
     (σ σ' : sReifier_state sR ♯ IT rs) β l :
     sReifier_re sR op (x, σ) ≡ Some (y, σ', l) →
     k (subEff_outs y) ≡ Next β →
-    has_substate rs σ
-    -∗ ▷ (£ 1 -∗ has_substate rs σ'
+    has_substate σ
+    -∗ ▷ (£ 1 -∗ has_substate σ'
           -∗ wp rs β s E1 Φ
-           ∗ ([∗ list] ef ∈ listO_map Tau l, wp rs ef s ⊤ (λ _ : ITV rs, True)))
+           ∗ wptp rs s (listO_map Tau l) (replicate (length (listO_map Tau l)) fork_post))
     -∗ wp rs (Vis (subEff_opid op) (subEff_ins x) k) s E1 Φ.
   Proof.
     intros HSR Hk.
@@ -1467,7 +1575,8 @@ Section weakestpre_specific.
   Qed.
 
   Lemma wp_subreify_ctx_indep_lift' a (rs : gReifiers a n)
-    `{!@stateG _ a rs A _ Σ} E1 s Φ sR
+    `{gitreeGS_gen n _ rs A Σ}
+    E1 s Φ sR
     `{!subReifier (sReifier_NotCtxDep_min sR a) rs}
     (op : opid (sReifier_ops sR))
     (x : Ins (sReifier_ops sR op) ♯ IT rs)
@@ -1476,10 +1585,10 @@ Section weakestpre_specific.
     (σ σ' : sReifier_state sR ♯ IT rs) β l :
     sReifier_re sR op (x, σ) ≡ Some (y, σ', l) →
     k (subEff_outs y) ≡ Next β →
-    has_substate rs σ
-    -∗ ▷ (£ 1 -∗ has_substate rs σ'
+    has_substate σ
+    -∗ ▷ (£ 1 -∗ has_substate σ'
           -∗ wp rs β s E1 Φ
-           ∗ ([∗ list] ef ∈ listO_map Tau l, wp rs ef s ⊤ (λ _ : ITV rs, True)))
+           ∗ wptp rs s (listO_map Tau l) (replicate (length (listO_map Tau l)) fork_post))
     -∗ wp rs (Vis (subEff_opid op) (subEff_ins x) k) s E1 Φ.
   Proof.
     destruct a.
@@ -1531,17 +1640,18 @@ Section weakestpre_specific.
   Qed.
 
   Lemma wp_subreify_ctx_indep_lift'' a (rs : gReifiers a n)
-    `{!@stateG _ a rs A _ Σ} E1 E2 s Φ sR
+    `{gitreeGS_gen n _ rs A Σ}
+    E1 E2 s Φ sR
     `{!subReifier (sReifier_NotCtxDep_min sR a) rs}
     (op : opid (sReifier_ops sR)) (x : Ins (sReifier_ops sR op) ♯ (IT rs))
     (k : Outs (F rs (subEff_opid op)) ♯ IT rs -n> laterO (IT rs)) :
     (|={E1,E2}=> ∃ σ y σ' β l,
-       has_substate rs σ ∗
+       has_substate σ ∗
          sReifier_re sR op (x, σ) ≡ Some (y, σ', l)
        ∗ k (subEff_outs y) ≡ Next β
-       ∗ ▷ (£ 1 -∗ has_substate rs σ'
-            ={E2,E1}=∗ wp rs β s E1 Φ ∗
-                       ([∗ list] ef ∈ listO_map Tau l, wp rs ef s ⊤ (λ _ : ITV rs, True))))
+       ∗ ▷ (£ 1 -∗ has_substate σ'
+            ={E2,E1}=∗ wp rs β s E1 Φ
+                     ∗ wptp rs s (listO_map Tau l) (replicate (length (listO_map Tau l)) fork_post)))
     -∗ wp rs (Vis (subEff_opid op) (subEff_ins x) k) s E1 Φ.
   Proof.
     destruct a.
@@ -1574,7 +1684,7 @@ Section weakestpre_specific.
     - iApply wp_subreify_ctx_indep'.
   Qed.
 
-End weakestpre_specific.
+End weakestpre_lifting.
 
 Section weakestpre_bind.
   Context {n : nat} (rs : gReifiers NotCtxDep n) {A} `{!Cofe A}.
@@ -1601,7 +1711,7 @@ Section weakestpre_bind.
   Implicit Type op : opid F.
   Implicit Type α β : IT.
 
-  Context `{!invGS Σ} `{!stateG rs (A:=A) Σ}.
+  Context `{!gitreeGS_gen rs A Σ}.
   Notation iProp := (iProp Σ).
   Notation coPsetO := (leibnizO coPset).
 
@@ -1622,8 +1732,10 @@ Section weakestpre_bind.
     destruct (IT_to_V (f α)) as [βv|] eqn:Hfa.
     - iLeft. iExists βv. iSplit; first done.
       assert (is_Some (IT_to_V α)) as [αv Ha].
-      { apply (IT_hom_val_inv _ f). rewrite Hfa.
-        done. }
+      {
+        apply (IT_hom_val_inv _ f). rewrite Hfa.
+        done.
+      }
       assert (IntoVal α αv).
       { apply IT_of_to_V'. by rewrite Ha. }
       rewrite wp_val_inv.
@@ -1632,16 +1744,18 @@ Section weakestpre_bind.
       rewrite IT_of_to_V'; last by rewrite -Hfa.
       by iApply fupd_wp.
     - iRight. iSplit; eauto.
-      iIntros (σ) "Hs".
+      iIntros (σ ns) "Hs".
       rewrite wp_unfold.
       iDestruct "H" as "[H | H]".
       + iDestruct "H" as (αv) "[Hav H]".
         iPoseProof (IT_of_to_V with "Hav") as "Hav".
         iMod "H" as "H". rewrite wp_unfold.
         iDestruct "H" as "[H|H]".
-        { iExFalso. iDestruct "H" as (βv) "[H _]".
+        {
+          iExFalso. iDestruct "H" as (βv) "[H _]".
           iRewrite "Hav" in "H". rewrite Hfa.
-          iApply (option_equivI with "H"). }
+          iApply (option_equivI with "H").
+        }
         iDestruct "H" as "[_ H]".
         iMod ("H" with "Hs") as "H". iModIntro.
         iRewrite "Hav" in "H". done.
@@ -1654,25 +1768,33 @@ Section weakestpre_bind.
             iExists (f α'), σ', l'. iApply (internal_step_hom with "Hsafe").
           - iDestruct "Herr" as (e) "[Herr %]".
             iRight. iExists e. iSplit; last done.
-            iRewrite "Herr". rewrite hom_err//. }
+            iRewrite "Herr". rewrite hom_err//.
+        }
         iIntros (σ' β l) "Hst".
         rewrite {1}internal_step_hom_inv. iDestruct "Hst" as "[%Ha | [_ Hst]]".
-        { destruct Ha as [αv Ha]. rewrite Ha.
+        {
+          destruct Ha as [αv Ha]. rewrite Ha.
           iExFalso.
-          iApply (option_equivI with "Hav"). }
+          iApply (option_equivI with "Hav").
+        }
         iDestruct "Hst" as (α') "[Hst Hb]".
         iIntros "Hlc".
+        iSimpl.
+        iSimpl in "H".
         iMod ("H" with "Hst Hlc") as "H". iModIntro.
         iNext. iMod "H" as "H". iModIntro.
-        iMod "H" as "[$ [H1 H2]]".
-        iModIntro. iRewrite "Hb".
+        iApply (step_fupdN_wand with "H").
+        iIntros ">H".
+        iModIntro.
+        iDestruct "H" as "[$ [H1 H2]]".
+        iRewrite "Hb".
         iSplitR "H2"; last done.
         by iApply "IH".
   Qed.
 
 End weakestpre_bind.
 
-Arguments wp {_ _} rs {_ _ _ _ _} α s E Φ.
+Arguments wp {_ _} rs {_ _ _ _} α s E Φ.
 Arguments has_full_state {n _ _ _ _ _ _} σ.
 Arguments has_state_idx {n _ _ _ _ _ _} i σ.
 Arguments has_substate {n _ _ _ _ _ _ _ _} σ.
@@ -1680,169 +1802,135 @@ Arguments stateG {n _} rs A {_} Σ.
 Arguments statePreG {n _} rs A {_} Σ.
 Arguments stateΣ {n _} rs A {_}.
 
-Definition notStuck : stuckness := λ e, False.
-
-Notation "'WP@{' re } α @ s ; E {{ Φ } }" :=
-  (wp re α s E Φ)
-    (at level 20, α, s, Φ at level 200, only parsing) : bi_scope.
-
-Notation "'WP@{' re } α @ s ; E {{ v , Q } }" :=
-  (wp re α s E (λ v, Q))
-    (at level 20, α, s, Q at level 200,
-      format "'[hv' 'WP@{' re }  α  '/' @  s  ;  E  '/' {{  '[' v ,  '/' Q  ']' } } ']'") : bi_scope.
-
-Notation "'WP@{' re } α @  s {{ β , Φ } }" :=
-  (wp re α s ⊤ (λ β, Φ))
-    (at level 20, α, Φ at level 200,
-      format "'WP@{' re }  α  @  s  {{  β ,  Φ  } }") : bi_scope.
-
-Notation "'WP@{' re } α  @  s {{ Φ } }" :=
-  (wp re α s ⊤ Φ)
-    (at level 20, α, Φ at level 200,
-      format "'WP@{' re }  α  @  s  {{  Φ  } }") : bi_scope.
-
-Notation "'WP@{' re } α {{ β , Φ } }" :=
-  (wp re α notStuck ⊤ (λ β, Φ))
-    (at level 20, α, Φ at level 200,
-      format "'WP@{' re }  α  {{  β ,  Φ  } }") : bi_scope.
-
-Notation "'WP@{' re } α {{ Φ } }" :=
-  (wp re α notStuck ⊤ Φ)
-    (at level 20, α, Φ at level 200,
-      format "'WP@{' re }  α  {{  Φ  } }") : bi_scope.
-
-Lemma wp_adequacy cr Σ `{!invGpreS Σ} n a (rs : gReifiers a n)
-  {A} `{!Cofe A} `{!statePreG rs A Σ}
-  (α : IT _ A) σ βv σ' s l k (ψ : (ITV (gReifiers_ops rs) A) → Prop) :
-  external_steps (gReifiers_sReifier rs) α σ (IT_of_V βv) σ' l k →
-  (∀ `{H1 : !invGS Σ} `{H2: !stateG rs A Σ},
-     ∃ Φ, NonExpansive Φ ∧ (∀ βv, Φ βv ⊢ ⌜ψ βv⌝)
-          ∧ (£ cr ∗ has_full_state σ ⊢ WP@{rs} α @ s {{ Φ }})%I)  →
-  ψ βv.
+Lemma wp_adequacy_tp (num_later_per_step : nat → nat)
+  n a (rs : gReifiers a n)
+  {A} `{!Cofe A}
+  Σ `{!invGpreS Σ} `{!statePreG rs A Σ}
+  α σ β σ' (s : stuckness) k ψ :
+  let rg := gReifiers_sReifier rs in
+  let F := sReifier_ops rg in
+  let IT := IT F A in
+  let ITV := ITV F A in
+  (∀ `{H1 : !invGS_gen HasLc Σ} `{H2 : !stateG rs A Σ},
+     (⊢@{iProp Σ} |={⊤}=> ∃
+                            (state_interp_fun
+                              : nat
+                                → (gReifiers_state rs) ♯ IT
+                                → iProp Σ)
+                            (aux_interp_fun : nat → iProp Σ)
+                            (fork_post : ITV -d> iProp Σ)
+                            fork_post_ne
+                            (Φs : list (ITV -d> iProp Σ))
+                            state_interp_fun_mono
+                            state_interp_fun_ne
+                            state_interp_fun_decomp,
+        let _ : gitreeGS_gen rs A Σ :=
+          GitreeG rs A Σ H1 H2
+            state_interp_fun aux_interp_fun
+            fork_post
+            fork_post_ne
+            num_later_per_step
+            state_interp_fun_mono
+            state_interp_fun_ne
+            state_interp_fun_decomp
+        in
+        tp_internal_steps (A := A) (gReifiers_sReifier rs) α σ β σ' k
+        ∗ state_interp_fun 0 σ
+        ∗ wptp rs s α Φs
+        ∗ (state_interp_fun k σ' -∗ |={⊤,∅}=> ⌜ ψ ⌝))%I)
+  → ψ.
 Proof.
-  intros Hst Hprf.
-  cut (⊢ ⌜ψ βv⌝ : iProp Σ)%I.
+  intros rg F IT' ITV' Hprf.
+  cut (⊢ ⌜ψ⌝ : iProp Σ)%I.
   { intros HH. eapply uPred.pure_soundness; eauto. }
-  eapply (step_fupdN_soundness_lc _ 0 (cr + 3*k)).
-  intros Hinv. iIntros "[Hcr Hlc]".
-  iMod (new_state_interp rs σ) as (sg) "[Hs Hs2]".
-  destruct (Hprf Hinv sg) as (Φ & HΦ & HΦψ & Hprf').
-  iPoseProof (Hprf' with "[$Hcr $Hs2]") as "Hic".
-  iPoseProof (wp_external_steps with "[$Hs $Hic]") as "Hphi".
-  { eassumption. }
-  iMod ("Hphi" with "Hlc") as "[Hst [H1 H2]]".
-  rewrite wp_val_inv; eauto.
-  iMod "H1" as "H1".
-  rewrite HΦψ. iFrame "H1".
-  by iApply fupd_mask_intro_discard.
+  eapply (step_fupdN_soundness_lc _ (steps_sum num_later_per_step 0 k)
+            (steps_sum num_later_per_step 0 k)).
+  intros Hinv. iIntros "Hcred".
+  iMod (new_state_interp σ) as (sg) "[Hs Hs2]".
+  specialize (Hprf Hinv sg).
+  iMod Hprf as (state_interp_fun aux_interp_fun
+                  fork_post
+                  fork_post_ne
+                  ?
+                  state_interp_fun_mono
+                  state_interp_fun_ne
+                  state_interp_fun_decomp)
+                 "(Hstep & Hσ & Hwp & H)".
+  iDestruct (big_sepL2_length with "Hwp") as %Hlen1.
+  iMod (@wptp_postconditions n a rs A _ Σ
+          (GitreeG rs A Σ _ _
+             state_interp_fun
+             aux_interp_fun
+             fork_post
+             fork_post_ne
+             num_later_per_step
+             state_interp_fun_mono
+             state_interp_fun_ne
+             state_interp_fun_decomp) _ _ s k α β σ
+          0 σ' with "Hstep Hσ Hcred Hwp") as "J".
+  iModIntro.
+  iApply (step_fupdN_wand with "J").
+  iIntros "J".
+  iEval (rewrite Nat.add_0_r) in "J".
+
 Qed.
 
-Lemma wp_adequacy_tp cr Σ `{!invGpreS Σ} n a (rs : gReifiers a n)
-  {A} `{!Cofe A} `{!statePreG rs A Σ}
-  (α : (IT _ A)) σ β βv σ' s k (ψ : (ITV (gReifiers_ops rs) A) → Prop) :
-  tp_external_steps (gReifiers_sReifier rs) [α] σ ((IT_of_V βv) :: β) σ' k →
-  (∀ `{H1 : !invGS Σ} `{H2: !stateG rs A Σ},
-     ∃ (Φs : list (ITV (gReifiers_ops rs) A -> iPropI Σ)),
-       (Forall (λ f, (∀ n, Proper (dist n ==> dist n) f)) Φs) ∧
-       (∀ βv, (from_option id (λ _, True%I) (head Φs)) βv ⊢ ⌜ψ βv⌝) ∧
-       (£ cr ∗ has_full_state σ ⊢ [∗ list] x;Φ ∈ [α];Φs, WP@{rs} x @ s {{ Φ }})%I)
-  → ψ βv.
-Proof.
-  intros Hst Hprf.
-  cut (⊢ ⌜ψ βv⌝ : iProp Σ)%I.
-  { intros HH. eapply uPred.pure_soundness; eauto. }
-  eapply (step_fupdN_soundness_lc _ 0 (cr + (k * k + 2 * k))).
-  intros Hinv. iIntros "[Hcr Hlc]".
-  iMod (new_state_interp rs σ) as (sg) "[Hs Hs2]".
-  destruct (Hprf Hinv sg) as (Φs & Hne & Hprf' & Hprf'').
-  iPoseProof (Hprf'' with "[$Hcr $Hs2]") as "Hic".
-  iPoseProof (wp_tp_external_steps with "[$Hs $Hic]") as "Hphi".
-  { eassumption. }
-  iMod ("Hphi" with "Hlc") as "[Hst H]".
-  simpl.
-  iDestruct "H" as "[H1  H2]".
-  rewrite take_0.
-  specialize (Hprf' βv).
-  iPoseProof (big_sepL2_alt with "H1") as "H1".
-  iDestruct "H1" as "[%HW1 HW2]".
-  simpl in HW1.
-  assert (∃ Φ, Φs = [Φ]) as HHH.
-  { destruct Φs as [| b ?].
-    - inversion HW1.
-    - simpl in HW1.
-      inversion HW1 as [HW2].
-      destruct Φs.
-      + exists b; done.
-      + inversion HW2.
-  }
-  destruct HHH as [Φ ->].
-  simpl.
-  iDestruct "HW2" as "[HW2 _]".
-  erewrite wp_val_inv; eauto.
-  - iMod "HW2" as "H".
-    iApply Hprf'.
-    simpl in *.
-    by iApply fupd_mask_intro_discard.
-  - by rewrite Forall_singleton in Hne.
-  - apply _.
-Qed.
-
-Lemma wp_safety cr Σ `{!invGpreS Σ} n a (rs : gReifiers a n)
-  {A} `{!Cofe A} `{!statePreG rs A Σ} s l k
-  (α β : IT (gReifiers_ops rs) A) (σ σ' : gReifiers_state rs ♯ IT (gReifiers_ops rs) A) :
-  (∀ Σ P Q, @disjunction_property Σ P Q) →
-  external_steps (gReifiers_sReifier rs) α σ β σ' l k →
-  IT_to_V β ≡ None →
-  (∀ `{H1 : !invGS_gen HasLc Σ} `{H2: !stateG rs A Σ},
-     ∃ Φ, NonExpansive Φ ∧ (£ cr ∗ has_full_state σ ⊢ WP@{rs} α @ s {{ Φ }})%I)  →
-  ((∃ β1 σ1 l1, external_step (gReifiers_sReifier rs) β σ' β1 σ1 l1)
-   ∨ (∃ e, β ≡ Err e ∧ s e)).
-Proof.
-  Opaque internal_step.
-  intros Hdisj Hstep Hbv Hwp.
-  cut (⊢@{iProp Σ} (∃ β1 σ1 l1, internal_step (gReifiers_sReifier rs) β σ' β1 σ1 l1)
-        ∨ (∃ e, β ≡ Err e ∧ ⌜s e⌝))%I.
-  { intros [Hprf | Hprf]%Hdisj.
-    - left.
-      apply (internal_step_safe_external_step _ (Σ:=Σ)).
-      { apply Hdisj. }
-      done.
-    - right.
-      destruct (IT_dont_confuse β)
-        as [[e Ha] | [[m Ha] | [ [g Ha] | [[α' Ha]|[op [i [ko Ha]]]] ]]].
-      + exists e. split; eauto.
-        eapply uPred.pure_soundness.
-        iPoseProof (Hprf) as "H".
-        iDestruct "H" as (e') "[He %Hs]". rewrite Ha.
-        iPoseProof (Err_inj' with "He") as "%He".
-        iPureIntro. rewrite He//.
-      + exfalso. eapply uPred.pure_soundness.
-        iPoseProof (Hprf) as "H".
-        iDestruct "H" as (e') "[Ha Hs]". rewrite Ha.
-        iApply (IT_ret_err_ne with "Ha").
-      + exfalso. eapply uPred.pure_soundness.
-        iPoseProof (Hprf) as "H".
-        iDestruct "H" as (e') "[Ha Hs]". rewrite Ha.
-        iApply (IT_fun_err_ne with "Ha").
-      + exfalso. eapply uPred.pure_soundness.
-        iPoseProof (Hprf) as "H".
-        iDestruct "H" as (e') "[Ha Hs]". rewrite Ha.
-        iApply (IT_tick_err_ne with "Ha").
-      + exfalso. eapply uPred.pure_soundness.
-        iPoseProof (Hprf) as "H".
-        iDestruct "H" as (e') "[Ha Hs]". rewrite Ha.
-        iApply (IT_vis_err_ne with "Ha"). }
-  eapply (step_fupdN_soundness_lc _ 0 (cr + (3*k+2))).
-  intros Hinv. iIntros "[Hcr Hlc]".
-  iMod (new_state_interp rs σ) as (sg) "[Hs Hs2]".
-  destruct (Hwp Hinv sg) as (Φ & HΦ & Hprf').
-  iPoseProof (Hprf' with "[$Hs2 $Hcr]") as "Hic".
-  iPoseProof (wp_external_steps_internal_safe with "[$Hs $Hic]") as "H".
-  { eassumption. }
-  iMod ("H" with "Hlc") as "[H | H]".
-  { iDestruct "H" as (βv) "%Hbeta".
-    exfalso. rewrite Hbeta  in Hbv.
-    inversion Hbv. }
-  iFrame "H".
-  by iApply fupd_mask_intro_discard.
-Qed.
+(* Lemma wp_safety cr Σ `{!invGpreS Σ} n a (rs : gReifiers a n) *)
+(*   {A} `{!Cofe A} `{!statePreG rs A Σ} s l k *)
+(*   (α β : IT (gReifiers_ops rs) A) (σ σ' : gReifiers_state rs ♯ IT (gReifiers_ops rs) A) : *)
+(*   (∀ Σ P Q, @disjunction_property Σ P Q) → *)
+(*   external_steps (gReifiers_sReifier rs) α σ β σ' l k → *)
+(*   IT_to_V β ≡ None → *)
+(*   (∀ `{H1 : !invGS_gen HasLc Σ} `{H2: !stateG rs A Σ}, *)
+(*      ∃ Φ, NonExpansive Φ ∧ (£ cr ∗ has_full_state σ ⊢ WP@{rs} α @ s {{ Φ }})%I)  → *)
+(*   ((∃ β1 σ1 l1, external_step (gReifiers_sReifier rs) β σ' β1 σ1 l1) *)
+(*    ∨ (∃ e, β ≡ Err e ∧ s e)). *)
+(* Proof. *)
+(*   Opaque internal_step. *)
+(*   intros Hdisj Hstep Hbv Hwp. *)
+(*   cut (⊢@{iProp Σ} (∃ β1 σ1 l1, internal_step (gReifiers_sReifier rs) β σ' β1 σ1 l1) *)
+(*         ∨ (∃ e, β ≡ Err e ∧ ⌜s e⌝))%I. *)
+(*   { intros [Hprf | Hprf]%Hdisj. *)
+(*     - left. *)
+(*       apply (internal_step_safe_external_step _ (Σ:=Σ)). *)
+(*       { apply Hdisj. } *)
+(*       done. *)
+(*     - right. *)
+(*       destruct (IT_dont_confuse β) *)
+(*         as [[e Ha] | [[m Ha] | [ [g Ha] | [[α' Ha]|[op [i [ko Ha]]]] ]]]. *)
+(*       + exists e. split; eauto. *)
+(*         eapply uPred.pure_soundness. *)
+(*         iPoseProof (Hprf) as "H". *)
+(*         iDestruct "H" as (e') "[He %Hs]". rewrite Ha. *)
+(*         iPoseProof (Err_inj' with "He") as "%He". *)
+(*         iPureIntro. rewrite He//. *)
+(*       + exfalso. eapply uPred.pure_soundness. *)
+(*         iPoseProof (Hprf) as "H". *)
+(*         iDestruct "H" as (e') "[Ha Hs]". rewrite Ha. *)
+(*         iApply (IT_ret_err_ne with "Ha"). *)
+(*       + exfalso. eapply uPred.pure_soundness. *)
+(*         iPoseProof (Hprf) as "H". *)
+(*         iDestruct "H" as (e') "[Ha Hs]". rewrite Ha. *)
+(*         iApply (IT_fun_err_ne with "Ha"). *)
+(*       + exfalso. eapply uPred.pure_soundness. *)
+(*         iPoseProof (Hprf) as "H". *)
+(*         iDestruct "H" as (e') "[Ha Hs]". rewrite Ha. *)
+(*         iApply (IT_tick_err_ne with "Ha"). *)
+(*       + exfalso. eapply uPred.pure_soundness. *)
+(*         iPoseProof (Hprf) as "H". *)
+(*         iDestruct "H" as (e') "[Ha Hs]". rewrite Ha. *)
+(*         iApply (IT_vis_err_ne with "Ha"). } *)
+(*   eapply (step_fupdN_soundness_lc _ 0 (cr + (3*k+2))). *)
+(*   intros Hinv. iIntros "[Hcr Hlc]". *)
+(*   iMod (new_state_interp rs σ) as (sg) "[Hs Hs2]". *)
+(*   destruct (Hwp Hinv sg) as (Φ & HΦ & Hprf'). *)
+(*   iPoseProof (Hprf' with "[$Hs2 $Hcr]") as "Hic". *)
+(*   iPoseProof (wp_external_steps_internal_safe with "[$Hs $Hic]") as "H". *)
+(*   { eassumption. } *)
+(*   iMod ("H" with "Hlc") as "[H | H]". *)
+(*   { iDestruct "H" as (βv) "%Hbeta". *)
+(*     exfalso. rewrite Hbeta  in Hbv. *)
+(*     inversion Hbv. } *)
+(*   iFrame "H". *)
+(*   by iApply fupd_mask_intro_discard. *)
+(* Qed. *)
