theories/lang_generic.v
@@ -67,277 +67,277 @@ Section ctx_interp.
 
 End ctx_interp.
 
-(* Common definitions and lemmas for Kripke logical relations *)
-Section kripke_logrel.
-  Variable s : stuckness.
+(* (* Common definitions and lemmas for Kripke logical relations *) *)
+(* Section kripke_logrel. *)
+(*   Variable s : stuckness. *)
 
-  Context {sz : nat} {a : is_ctx_dep}.
-  Variable rs : gReifiers a sz.
-  Context {R} `{!Cofe R}.
+(*   Context {sz : nat} {a : is_ctx_dep}. *)
+(*   Variable rs : gReifiers a sz. *)
+(*   Context {R} `{!Cofe R}. *)
 
-  Notation F := (gReifiers_ops rs).
-  Notation IT := (IT F R).
-  Notation ITV := (ITV F R).
-  Context `{!invGS Σ, !stateG rs R Σ}.
-  Notation iProp := (iProp Σ).
+(*   Notation F := (gReifiers_ops rs). *)
+(*   Notation IT := (IT F R). *)
+(*   Notation ITV := (ITV F R). *)
+(*   Context `{!invGS Σ, !stateG rs R Σ}. *)
+(*   Notation iProp := (iProp Σ). *)
 
-  Context {A:ofe}. (* The type & predicate for the explicit Kripke worlds *)
-  Variable (P : A -n> iProp).
+(*   Context {A:ofe}. (* The type & predicate for the explicit Kripke worlds *) *)
+(*   Variable (P : A -n> iProp). *)
 
-  Implicit Types α β : IT.
-  Implicit Types αv βv : ITV.
-  Implicit Types Φ Ψ : ITV -n> iProp.
+(*   Implicit Types α β : IT. *)
+(*   Implicit Types αv βv : ITV. *)
+(*   Implicit Types Φ Ψ : ITV -n> iProp. *)
 
-  Program Definition expr_pred (α : IT) (Φ : ITV -n> iProp) : iProp :=
-    (∀ x : A, P x -∗ wp rs α s ⊤ (λne v, ∃ y : A, Φ v ∗ P y)).
-  Next Obligation.
-    solve_proper.
-  Qed.
+(*   Program Definition expr_pred (α : IT) (Φ : ITV -n> iProp) : iProp := *)
+(*     (∀ x : A, P x -∗ wp rs α s ⊤ (λne v, ∃ y : A, Φ v ∗ P y)). *)
+(*   Next Obligation. *)
+(*     solve_proper. *)
+(*   Qed. *)
 
-  Global Instance expr_pred_ne {n} : Proper (dist n ==> dist n ==> dist n) expr_pred.
-  Proof.
-    intros ??????.
-    unfold expr_pred.
-    simpl.
-    f_equiv.
-    intros ?; simpl.
-    f_equiv.
-    f_equiv; first done.
-    intros ?; simpl.
-    f_equiv.
-    intros ?; simpl.
-    solve_proper.
-  Qed.
+(*   Global Instance expr_pred_ne {n} : Proper (dist n ==> dist n ==> dist n) expr_pred. *)
+(*   Proof. *)
+(*     intros ??????. *)
+(*     unfold expr_pred. *)
+(*     simpl. *)
+(*     f_equiv. *)
+(*     intros ?; simpl. *)
+(*     f_equiv. *)
+(*     f_equiv; first done. *)
+(*     intros ?; simpl. *)
+(*     f_equiv. *)
+(*     intros ?; simpl. *)
+(*     solve_proper. *)
+(*   Qed. *)
 
-  Global Instance expr_pred_proper : Proper (equiv ==> equiv ==> equiv) expr_pred.
-  Proof.
-    intros ??????.
-    unfold expr_pred.
-    simpl.
-    f_equiv.
-    intros ?; simpl.
-    f_equiv.
-    f_equiv; first done.
-    intros ?; simpl.
-    f_equiv.
-    intros ?; simpl.
-    solve_proper.
-  Qed.
+(*   Global Instance expr_pred_proper : Proper (equiv ==> equiv ==> equiv) expr_pred. *)
+(*   Proof. *)
+(*     intros ??????. *)
+(*     unfold expr_pred. *)
+(*     simpl. *)
+(*     f_equiv. *)
+(*     intros ?; simpl. *)
+(*     f_equiv. *)
+(*     f_equiv; first done. *)
+(*     intros ?; simpl. *)
+(*     f_equiv. *)
+(*     intros ?; simpl. *)
+(*     solve_proper. *)
+(*   Qed. *)
 
-  Lemma expr_pred_ret α αv Φ `{!IntoVal α αv} :
-    Φ αv ⊢ expr_pred α Φ.
-  Proof.
-    iIntros "H".
-    iIntros (x) "Hx". iApply wp_val.
-    simpl.
-    iExists x.
-    by iFrame.
-  Qed.
+(*   Lemma expr_pred_ret α αv Φ `{!IntoVal α αv} : *)
+(*     Φ αv ⊢ expr_pred α Φ. *)
+(*   Proof. *)
+(*     iIntros "H". *)
+(*     iIntros (x) "Hx". iApply wp_val. *)
+(*     simpl. *)
+(*     iExists x. *)
+(*     by iFrame. *)
+(*   Qed. *)
 
-  Lemma expr_pred_frame α Φ :
-    WP@{rs} α @ s {{ Φ }} ⊢ expr_pred α Φ.
-  Proof.
-    iIntros "H".
-    iIntros (x) "Hx".
-    iApply (wp_wand with "H").
-    simpl.
-    iIntros (v) "Hv".
-    iExists x.
-    by iFrame.
-  Qed.
+(*   Lemma expr_pred_frame α Φ : *)
+(*     WP@{rs} α @ s {{ Φ }} ⊢ expr_pred α Φ. *)
+(*   Proof. *)
+(*     iIntros "H". *)
+(*     iIntros (x) "Hx". *)
+(*     iApply (wp_wand with "H"). *)
+(*     simpl. *)
+(*     iIntros (v) "Hv". *)
+(*     iExists x. *)
+(*     by iFrame. *)
+(*   Qed. *)
 
-End kripke_logrel.
+(* End kripke_logrel. *)
 
-Section kripke_logrel_ctx_indep.
-  Variable s : stuckness.
+(* Section kripke_logrel_ctx_indep. *)
+(*   Variable s : stuckness. *)
 
-  Context {sz : nat}.
-  Variable rs : gReifiers NotCtxDep sz.
-  Context {R} `{!Cofe R}.
+(*   Context {sz : nat}. *)
+(*   Variable rs : gReifiers NotCtxDep sz. *)
+(*   Context {R} `{!Cofe R}. *)
 
-  Notation F := (gReifiers_ops rs).
-  Notation IT := (IT F R).
-  Notation ITV := (ITV F R).
-  Context `{!invGS Σ, !stateG rs R Σ}.
-  Notation iProp := (iProp Σ).
+(*   Notation F := (gReifiers_ops rs). *)
+(*   Notation IT := (IT F R). *)
+(*   Notation ITV := (ITV F R). *)
+(*   Context `{!invGS Σ, !stateG rs R Σ}. *)
+(*   Notation iProp := (iProp Σ). *)
 
-  Context {A : ofe}.
-  Variable (P : A -n> iProp).
+(*   Context {A : ofe}. *)
+(*   Variable (P : A -n> iProp). *)
 
-  Implicit Types α β : IT.
-  Implicit Types αv βv : ITV.
-  Implicit Types Φ Ψ : ITV -n> iProp.
+(*   Implicit Types α β : IT. *)
+(*   Implicit Types αv βv : ITV. *)
+(*   Implicit Types Φ Ψ : ITV -n> iProp. *)
 
-  Local Notation expr_pred := (expr_pred s rs P).
+(*   Local Notation expr_pred := (expr_pred s rs P). *)
 
-  Lemma expr_pred_bind f `{!IT_hom f} α Φ Ψ `{!NonExpansive Φ}
-    : expr_pred α Ψ ⊢
-      (∀ αv, Ψ αv -∗ expr_pred (f (IT_of_V αv)) Φ)
-      -∗ expr_pred (f α) Φ.
-  Proof.
-    iIntros "H1 H2".
-    iIntros (x) "Hx".
-    iApply wp_bind.
-    iSpecialize ("H1" with "Hx").
-    iApply (wp_wand with "H1").
-    iIntros (βv). iDestruct 1 as (y) "[Hb Hy]".
-    iModIntro.
-    iApply ("H2" with "Hb Hy").
-  Qed.
-End kripke_logrel_ctx_indep.
+(*   Lemma expr_pred_bind f `{!IT_hom f} α Φ Ψ `{!NonExpansive Φ} *)
+(*     : expr_pred α Ψ ⊢ *)
+(*       (∀ αv, Ψ αv -∗ expr_pred (f (IT_of_V αv)) Φ) *)
+(*       -∗ expr_pred (f α) Φ. *)
+(*   Proof. *)
+(*     iIntros "H1 H2". *)
+(*     iIntros (x) "Hx". *)
+(*     iApply wp_bind. *)
+(*     iSpecialize ("H1" with "Hx"). *)
+(*     iApply (wp_wand with "H1"). *)
+(*     iIntros (βv). iDestruct 1 as (y) "[Hb Hy]". *)
+(*     iModIntro. *)
+(*     iApply ("H2" with "Hb Hy"). *)
+(*   Qed. *)
+(* End kripke_logrel_ctx_indep. *)
 
-Arguments expr_pred_bind {_ _ _ _ _ _ _ _ _ _} f {_ _}.
+(* Arguments expr_pred_bind {_ _ _ _ _ _ _ _ _ _} f {_ _}. *)
 
-Section tm_interp.
-  Context {sz : nat} {a : is_ctx_dep}.
-  Variable rs : gReifiers a sz.
-  Context {R} `{!Cofe R}.
+(* Section tm_interp. *)
+(*   Context {sz : nat} {a : is_ctx_dep}. *)
+(*   Variable rs : gReifiers a sz. *)
+(*   Context {R} `{!Cofe R}. *)
 
-  Notation F := (gReifiers_ops rs).
-  Notation IT := (IT F R).
-  Notation ITV := (ITV F R).
-  Context `{!invGS Σ, !stateG rs R Σ}.
-  Notation iProp := (iProp Σ).
+(*   Notation F := (gReifiers_ops rs). *)
+(*   Notation IT := (IT F R). *)
+(*   Notation ITV := (ITV F R). *)
+(*   Context `{!invGS Σ, !stateG rs R Σ}. *)
+(*   Notation iProp := (iProp Σ). *)
 
-  Context {A : ofe}.
-  Variable (P : A -n> iProp).
+(*   Context {A : ofe}. *)
+(*   Variable (P : A -n> iProp). *)
 
-  Variable (ty : Set).
-  Variable (interp_ty : ty → (ITV -n> iProp)).
-  Variable (kripke : IT → (ITV -n> iProp) → iProp).
+(*   Variable (ty : Set). *)
+(*   Variable (interp_ty : ty → (ITV -n> iProp)). *)
+(*   Variable (kripke : IT → (ITV -n> iProp) → iProp). *)
 
-  Definition ssubst_valid1 {S : Set}
-    (Γ : S -> ty)
-    (ss : interp_scope S) : iProp :=
-    (∀ x, □ kripke (ss x) (interp_ty (Γ x)))%I.
+(*   Definition ssubst_valid1 {S : Set} *)
+(*     (Γ : S -> ty) *)
+(*     (ss : interp_scope S) : iProp := *)
+(*     (∀ x, □ kripke (ss x) (interp_ty (Γ x)))%I. *)
 
-  Global Instance ssubst_valid_pers `{∀ τ β, Persistent (interp_ty τ β)}
-    {S : Set} (Γ : S → ty) ss : Persistent (ssubst_valid1 Γ ss).
-  Proof. apply _. Qed.
+(*   Global Instance ssubst_valid_pers `{∀ τ β, Persistent (interp_ty τ β)} *)
+(*     {S : Set} (Γ : S → ty) ss : Persistent (ssubst_valid1 Γ ss). *)
+(*   Proof. apply _. Qed. *)
 
-End tm_interp.
+(* End tm_interp. *)
 
-Section tm_interp_fin.
-  Context {sz : nat} {a : is_ctx_dep}.
-  Variable rs : gReifiers a sz.
-  Context {R} `{!Cofe R}.
+(* Section tm_interp_fin. *)
+(*   Context {sz : nat} {a : is_ctx_dep}. *)
+(*   Variable rs : gReifiers a sz. *)
+(*   Context {R} `{!Cofe R}. *)
 
-  Notation F := (gReifiers_ops rs).
-  Notation IT := (IT F R).
-  Notation ITV := (ITV F R).
-  Context `{!invGS Σ, !stateG rs R Σ}.
-  Notation iProp := (iProp Σ).
+(*   Notation F := (gReifiers_ops rs). *)
+(*   Notation IT := (IT F R). *)
+(*   Notation ITV := (ITV F R). *)
+(*   Context `{!invGS Σ, !stateG rs R Σ}. *)
+(*   Notation iProp := (iProp Σ). *)
 
-  Context {A : ofe}.
-  Variable (P : A -n> iProp).
+(*   Context {A : ofe}. *)
+(*   Variable (P : A -n> iProp). *)
 
-  Variable (ty : Set).
-  Variable (interp_ty : ty → (ITV -n> iProp)).
-  Variable (kripke : IT → (ITV -n> iProp) → iProp).
+(*   Variable (ty : Set). *)
+(*   Variable (interp_ty : ty → (ITV -n> iProp)). *)
+(*   Variable (kripke : IT → (ITV -n> iProp) → iProp). *)
 
-  Program Definition ssubst_valid_fin1 {S : Set} `{!EqDecision S} `{!Finite S}
-    (Ω : S → ty) (ss : interp_scope S) : iProp
-    := ([∗ set] x ∈ (fin_to_set S),
-         (kripke (ss x) (interp_ty (Ω x)))%I).
+(*   Program Definition ssubst_valid_fin1 {S : Set} `{!EqDecision S} `{!Finite S} *)
+(*     (Ω : S → ty) (ss : interp_scope S) : iProp *)
+(*     := ([∗ set] x ∈ (fin_to_set S), *)
+(*          (kripke (ss x) (interp_ty (Ω x)))%I). *)
 
-  Context (Q : iProp).
+(*   Context (Q : iProp). *)
 
-  Definition valid_fin1 {S : Set} `{!EqDecision S} `{!Finite S} (Ω : S → ty)
-    (α : interp_scope S -n> IT) (τ : ty) : iProp :=
-    ∀ ss, Q
-          -∗ (ssubst_valid_fin1 Ω ss)
-          -∗ kripke (α ss) (interp_ty τ).
+(*   Definition valid_fin1 {S : Set} `{!EqDecision S} `{!Finite S} (Ω : S → ty) *)
+(*     (α : interp_scope S -n> IT) (τ : ty) : iProp := *)
+(*     ∀ ss, Q *)
+(*           -∗ (ssubst_valid_fin1 Ω ss) *)
+(*           -∗ kripke (α ss) (interp_ty τ). *)
 
-  Lemma ssubst_valid_fin_empty1 (αs : interp_scope ∅) :
-    ⊢ ssubst_valid_fin1 □ αs.
-  Proof.
-    iStartProof.
-    unfold ssubst_valid_fin1.
-    rewrite fin_to_set_empty.
-    by iApply big_sepS_empty.
-  Qed.
+(*   Lemma ssubst_valid_fin_empty1 (αs : interp_scope ∅) : *)
+(*     ⊢ ssubst_valid_fin1 □ αs. *)
+(*   Proof. *)
+(*     iStartProof. *)
+(*     unfold ssubst_valid_fin1. *)
+(*     rewrite fin_to_set_empty. *)
+(*     by iApply big_sepS_empty. *)
+(*   Qed. *)
 
-  Lemma ssubst_valid_fin_app1
-    {S1 S2 : Set} `{!EqDecision S1} `{!Finite S1}
-    `{!EqDecision S2} `{!Finite S2}
-    `{!EqDecision (S1 + S2)} `{!Finite (S1 + S2)}
-    (Ω1 : S1 → ty) (Ω2 : S2 → ty)
-    (αs : interp_scope (sum S1 S2)) :
-    (ssubst_valid_fin1 (sum_map' Ω1 Ω2) αs) ⊢
-    (ssubst_valid_fin1 Ω1 (interp_scope_split αs).1)
-    ∗ (ssubst_valid_fin1 Ω2 (interp_scope_split αs).2).
-  Proof.
-    iIntros "H".
-    rewrite /ssubst_valid_fin1 fin_to_set_sum big_sepS_union; first last.
-    {
-      apply elem_of_disjoint.
-      intros [x | x].
-      - rewrite !elem_of_list_to_set.
-        intros _ H2.
-        apply elem_of_list_fmap_2 in H2.
-        destruct H2 as [y [H2 H2']]; inversion H2.
-      - rewrite !elem_of_list_to_set.
-        intros H1 _.
-        apply elem_of_list_fmap_2 in H1.
-        destruct H1 as [y [H1 H1']]; inversion H1.
-    }
-    iDestruct "H" as "(H1 & H2)".
-    iSplitL "H1".
-    - rewrite big_opS_list_to_set; first last.
-      {
-        apply NoDup_fmap.
-        - intros ??; by inversion 1.
-        - apply NoDup_elements.
-      }
-      rewrite big_sepL_fmap /=.
-      rewrite big_sepS_elements.
-      iFrame "H1".
-    - rewrite big_opS_list_to_set; first last.
-      {
-        apply NoDup_fmap.
-        - intros ??; by inversion 1.
-        - apply NoDup_elements.
-      }
-      rewrite big_sepL_fmap /=.
-      rewrite big_sepS_elements.
-      iFrame "H2".
-  Qed.
+(*   Lemma ssubst_valid_fin_app1 *)
+(*     {S1 S2 : Set} `{!EqDecision S1} `{!Finite S1} *)
+(*     `{!EqDecision S2} `{!Finite S2} *)
+(*     `{!EqDecision (S1 + S2)} `{!Finite (S1 + S2)} *)
+(*     (Ω1 : S1 → ty) (Ω2 : S2 → ty) *)
+(*     (αs : interp_scope (sum S1 S2)) : *)
+(*     (ssubst_valid_fin1 (sum_map' Ω1 Ω2) αs) ⊢ *)
+(*     (ssubst_valid_fin1 Ω1 (interp_scope_split αs).1) *)
+(*     ∗ (ssubst_valid_fin1 Ω2 (interp_scope_split αs).2). *)
+(*   Proof. *)
+(*     iIntros "H". *)
+(*     rewrite /ssubst_valid_fin1 fin_to_set_sum big_sepS_union; first last. *)
+(*     { *)
+(*       apply elem_of_disjoint. *)
+(*       intros [x | x]. *)
+(*       - rewrite !elem_of_list_to_set. *)
+(*         intros _ H2. *)
+(*         apply elem_of_list_fmap_2 in H2. *)
+(*         destruct H2 as [y [H2 H2']]; inversion H2. *)
+(*       - rewrite !elem_of_list_to_set. *)
+(*         intros H1 _. *)
+(*         apply elem_of_list_fmap_2 in H1. *)
+(*         destruct H1 as [y [H1 H1']]; inversion H1. *)
+(*     } *)
+(*     iDestruct "H" as "(H1 & H2)". *)
+(*     iSplitL "H1". *)
+(*     - rewrite big_opS_list_to_set; first last. *)
+(*       { *)
+(*         apply NoDup_fmap. *)
+(*         - intros ??; by inversion 1. *)
+(*         - apply NoDup_elements. *)
+(*       } *)
+(*       rewrite big_sepL_fmap /=. *)
+(*       rewrite big_sepS_elements. *)
+(*       iFrame "H1". *)
+(*     - rewrite big_opS_list_to_set; first last. *)
+(*       { *)
+(*         apply NoDup_fmap. *)
+(*         - intros ??; by inversion 1. *)
+(*         - apply NoDup_elements. *)
+(*       } *)
+(*       rewrite big_sepL_fmap /=. *)
+(*       rewrite big_sepS_elements. *)
+(*       iFrame "H2". *)
+(*   Qed. *)
 
-  Lemma ssubst_valid_fin_cons1 {S : Set} `{!EqDecision S} `{!Finite S}
-    (Ω : S → ty) (αs : interp_scope S) τ t :
-    ssubst_valid_fin1 Ω αs ∗ kripke t (interp_ty τ) ⊢ ssubst_valid_fin1 (Ω ▹ τ) (extend_scope αs t).
-  Proof.
-    iIntros "(H & G)".
-    rewrite /ssubst_valid_fin1.
-    rewrite fin_to_set_inc /=.
-    rewrite big_sepS_union; first last.
-    {
-      apply elem_of_disjoint.
-      intros [| x].
-      - rewrite !elem_of_list_to_set.
-        intros _ H2.
-        apply elem_of_list_fmap_2 in H2.
-        destruct H2 as [y [H2 H2']]; inversion H2.
-      - rewrite !elem_of_list_to_set.
-        intros H1 _.
-        apply elem_of_singleton_1 in H1.
-        inversion H1.
-    }
-    iSplitL "G".
-    - rewrite big_opS_singleton.
-      iFrame "G".
-    - erewrite big_opS_set_map.
-      + iFrame "H".
-      + intros ?? H; by inversion H.
-  Qed.
+(*   Lemma ssubst_valid_fin_cons1 {S : Set} `{!EqDecision S} `{!Finite S} *)
+(*     (Ω : S → ty) (αs : interp_scope S) τ t : *)
+(*     ssubst_valid_fin1 Ω αs ∗ kripke t (interp_ty τ) ⊢ ssubst_valid_fin1 (Ω ▹ τ) (extend_scope αs t). *)
+(*   Proof. *)
+(*     iIntros "(H & G)". *)
+(*     rewrite /ssubst_valid_fin1. *)
+(*     rewrite fin_to_set_inc /=. *)
+(*     rewrite big_sepS_union; first last. *)
+(*     { *)
+(*       apply elem_of_disjoint. *)
+(*       intros [| x]. *)
+(*       - rewrite !elem_of_list_to_set. *)
+(*         intros _ H2. *)
+(*         apply elem_of_list_fmap_2 in H2. *)
+(*         destruct H2 as [y [H2 H2']]; inversion H2. *)
+(*       - rewrite !elem_of_list_to_set. *)
+(*         intros H1 _. *)
+(*         apply elem_of_singleton_1 in H1. *)
+(*         inversion H1. *)
+(*     } *)
+(*     iSplitL "G". *)
+(*     - rewrite big_opS_singleton. *)
+(*       iFrame "G". *)
+(*     - erewrite big_opS_set_map. *)
+(*       + iFrame "H". *)
+(*       + intros ?? H; by inversion H. *)
+(*   Qed. *)
 
-  Lemma ssubst_valid_fin_lookup1 {S : Set} `{!EqDecision S} `{!Finite S}
-    (Ω : S → ty) (αs : interp_scope S) x :
-    ssubst_valid_fin1 Ω αs ⊢ kripke (αs x) (interp_ty (Ω x)).
-  Proof.
-    iIntros "H".
-    iDestruct (big_sepS_elem_of_acc _ _ x with "H") as "($ & _)";
-      first apply elem_of_fin_to_set.
-  Qed.
+(*   Lemma ssubst_valid_fin_lookup1 {S : Set} `{!EqDecision S} `{!Finite S} *)
+(*     (Ω : S → ty) (αs : interp_scope S) x : *)
+(*     ssubst_valid_fin1 Ω αs ⊢ kripke (αs x) (interp_ty (Ω x)). *)
+(*   Proof. *)
+(*     iIntros "H". *)
+(*     iDestruct (big_sepS_elem_of_acc _ _ x with "H") as "($ & _)"; *)
+(*       first apply elem_of_fin_to_set. *)
+(*   Qed. *)
 
-End tm_interp_fin.
+(* End tm_interp_fin. *)
